DY/SignedDH.lean
@@ -1,179 +1,97 @@
-import DY.Trace
-import DY.Step
-import DY.Bytes
-import DY.EquationalTheory.Literal
-import DY.EquationalTheory.Concat
-import DY.EquationalTheory.Hash
-import DY.EquationalTheory.Sign
-import DY.EquationalTheory.DiffieHellman
+module
+
+public import DY.Trace
+public import DY.Step
+public import DY.Bytes
+public import DY.EquationalTheory.Literal
+public import DY.EquationalTheory.Concat
+public import DY.EquationalTheory.Hash
+public import DY.EquationalTheory.Sign
+public import DY.EquationalTheory.DiffieHellman
+public import DY.Actions.Network
+public import DY.Actions.Random
+public import DY.Actions.ProtocolEvent
+public import DY.Actions.PersistentLocalState
+public import DY.Actions.LongTermKeys
+public import DY.Comparse
+import DY.Step.Utils
 
 open DY
+open DY.Comparse -- TODO?
+
+@[expose] public section
 
 namespace Test
 
 variable [BytesFunctor]
-variable [BytesFunctor.Has Hash.SubF]
-variable [BytesFunctor.Has DiffieHellman.SubF]
-variable [BytesFunctor.Has Signature.SubF]
 
-instance:
-  HoareTriple
-    (pure x: Traceful a)
-    (fun _ => True)
-    (fun res _ => res = x)
-  where
-    pf := sorry
+structure ClientInitiateState where
+  xPk: Bytes
+  xSk: Bytes
 
-instance:
-  HoareTriple
-    (OptionT.fail: Traceful a)
-    (fun _ => True)
-    (fun _ _ => True)
-  where
-    pf := sorry
+noncomputable
+instance: ParseableSerializeable ClientInitiateState := comparseMetaProgramExists
 
-def Principal := String
+axiom ClientInitiateState.isWellFormedLemma
+  (pre: Bytes → τ → Prop) [BytesCompatible pre] (x: ClientInitiateState) (tr: τ):
+  isWellFormed pre x tr = (pre x.xPk tr ∧ pre x.xSk tr)
 
-class ParseableSerializeable (a: Type) where
-  parse: Bytes -> Err a
-  serialize: a -> Bytes
+grind_pattern ClientInitiateState.isWellFormedLemma => isWellFormed pre x tr
 
-  parse_serialize_inv:
-    ∀ x: a,
-      parse (serialize x) = some x
+structure ClientFinishState where
+  xPk: Bytes
+  kC: Bytes
 
-  serialize_parse_inv:
-    ∀ buf: Bytes, ∀ x: a,
-      parse buf = some x →
-      buf = serialize x
+noncomputable
+instance: ParseableSerializeable ClientFinishState := comparseMetaProgramExists
 
-open ParseableSerializeable
+axiom ClientFinishState.isWellFormedLemma
+  (pre: Bytes → τ → Prop) [BytesCompatible pre] (x: ClientFinishState) (tr: τ):
+  isWellFormed pre x tr = (pre x.xPk tr ∧ pre x.kC tr)
 
-axiom comparseExists {a: Type}: ParseableSerializeable a
+grind_pattern ClientFinishState.isWellFormedLemma => isWellFormed pre x tr
 
-@[simp]
-theorem parse_serialize_inv_grind [ParseableSerializeable a] (x: a):
-  ParseableSerializeable.parse (serialize x) = some x
-  := by
-  exact (parse_serialize_inv x)
+structure ServerFinishState where
+  yPk: Bytes
+  kS: Bytes
 
-grind_pattern parse_serialize_inv_grind => serialize x
+noncomputable
+instance: ParseableSerializeable ServerFinishState := comparseMetaProgramExists
 
-def formatRel [ParseableSerializeable a] (buf: Bytes) (x: a) :=
-  buf = serialize x
+axiom ServerFinishState.isWellFormedLemma
+  (pre: Bytes → τ → Prop) [BytesCompatible pre] (x: ServerFinishState) (tr: τ):
+  isWellFormed pre x tr = (pre x.yPk tr ∧ pre x.kS tr)
 
-instance [ParseableSerializeable a]:
-  HoareTriple
-    (parse buf: Err a)
-    (fun _ => True)
-    (fun res _ => formatRel buf res)
-where
-  pf := by
-    simp only [hoareTriple, wp, formatRel, OptionT.run]
-    grind [serialize_parse_inv]
+grind_pattern ServerFinishState.isWellFormedLemma => isWellFormed pre x tr
 
-theorem serialize_formatRel [ParseableSerializeable a] (x: a):
-  (formatRel (serialize x) x)
-  := by
-    simp [formatRel]
-
-grind_pattern serialize_formatRel => serialize x
+-- TODO move
 grind_pattern [grind_later] serialize_formatRel => serialize x
-
-@[grind! .]
-theorem parse_formatRel [ParseableSerializeable a] (b: Bytes):
-  match (parse b: Err a) with
-  | none => True
-  | some x => formatRel b x
-  := by
-    grind [formatRel, serialize_parse_inv]
-
-def isWellFormed [ParseableSerializeable a] (pre: Bytes → τ → Prop) (x: a) (tr: τ): Prop :=
-  pre (serialize x) tr
-
-theorem isWellFormedFormatRel [ParseableSerializeable a] (pre: Bytes → τ → Prop) (buf: Bytes) (x: a) (tr: τ):
-  formatRel buf x →
-  (pre buf tr = isWellFormed pre x tr)
-  := by
-    grind [isWellFormed, formatRel]
-
-theorem isWellFormedFormatRelBytesWellFormed [BytesWellFormed] [ParseableSerializeable a]:
-  ∀ (buf: Bytes) (x: a) (tr: ProofTrace),
-  formatRel buf x →
-  (buf.WellFormed tr = isWellFormed Bytes.WellFormed x tr)
-  := isWellFormedFormatRel Bytes.WellFormed
-
-grind_pattern isWellFormedFormatRelBytesWellFormed => formatRel buf x, buf.WellFormed tr
-
-theorem isWellFormedFormatRelBytesInvariant [BytesInvariant] [ParseableSerializeable a]:
-  ∀ (buf: Bytes) (x: a) (tr: ProofTrace),
-  formatRel buf x →
-  (buf.Invariant tr = isWellFormed Bytes.Invariant x tr)
-  := isWellFormedFormatRel Bytes.Invariant
-
-grind_pattern isWellFormedFormatRelBytesInvariant => formatRel buf x, buf.Invariant tr
 grind_pattern [grind_later] isWellFormedFormatRelBytesInvariant => formatRel buf x, buf.Invariant tr
 
-theorem isWellFormedFormatRelIsPublishable [BytesInvariants] [ParseableSerializeable a]:
-  ∀ (buf: Bytes) (x: a) (tr: ProofTrace),
-  formatRel buf x →
-  (buf.Publishable tr = isWellFormed Bytes.Publishable x tr)
-  := isWellFormedFormatRel Bytes.Publishable
-
-grind_pattern isWellFormedFormatRelIsPublishable => formatRel buf x, Bytes.Publishable buf tr
-
-theorem isWellFormedParse [ParseableSerializeable a] (pre: Bytes → τ → Prop) (buf: Bytes) (x: a) (tr: τ):
-  parse buf = some x →
-  pre buf tr →
-  isWellFormed pre x tr
-  := by
-    grind [isWellFormed, serialize_parse_inv]
-
-class BytesCompatible (pre: Bytes → τ → Prop) where
-  dummy: Unit
-
-instance [BytesWellFormed]: BytesCompatible Bytes.WellFormed where
-  dummy := ()
-
-instance [BytesInvariant]: BytesCompatible Bytes.Invariant where
-  dummy := ()
-
-instance [BytesInvariants]: BytesCompatible Bytes.Publishable where
-  dummy := ()
-
-inductive ClientState where
-  | ClientInitiateState (x_sk: Bytes)
-  | ClientFinishState (k_c: Bytes)
-
-instance : ParseableSerializeable ClientState := sorry
-
-inductive ServerState where
-  | ServerFinishState (k_s: Bytes)
-
-instance : ParseableSerializeable ServerState := sorry
-
 structure ClientMessage where
-  x_pk: Bytes
+  xPk: Bytes
 
-instance : ParseableSerializeable ClientMessage := sorry
+noncomputable
+instance: ParseableSerializeable ClientMessage := comparseMetaProgramExists
 
 axiom ClientMessage.isWellFormedLemma
   (pre: Bytes → τ → Prop) [BytesCompatible pre] (x: ClientMessage) (tr: τ):
-  isWellFormed pre x tr = pre x.x_pk tr
+  isWellFormed pre x tr = pre x.xPk tr
 
 grind_pattern ClientMessage.isWellFormedLemma => isWellFormed pre x tr
 grind_pattern [grind_later] ClientMessage.isWellFormedLemma => isWellFormed pre x tr
 
 structure ServerMessage where
-  y_pk: Bytes
+  yPk: Bytes
   sig: Bytes
 
-instance : ParseableSerializeable ServerMessage := sorry
+noncomputable
+instance: ParseableSerializeable ServerMessage := comparseMetaProgramExists
 
 axiom ServerMessage.isWellFormedLemma
   (pre: Bytes → τ → Prop) [BytesCompatible pre] (x: ServerMessage) (tr: τ):
   isWellFormed pre x tr = (
-    pre x.y_pk tr ∧
+    pre x.yPk tr ∧
     pre x.sig tr
   )
 
@@ -181,74 +99,102 @@ grind_pattern ServerMessage.isWellFormedLemma => isWellFormed pre x tr
 grind_pattern [grind_later] ServerMessage.isWellFormedLemma => isWellFormed pre x tr
 
 structure SigInput where
-  x_pk: Bytes
-  y_pk: Bytes
+  xPk: Bytes
+  yPk: Bytes
 
 noncomputable
-instance: ParseableSerializeable SigInput := comparseExists
+instance: ParseableSerializeable SigInput := comparseMetaProgramExists
 
 axiom SigInput.isWellFormedLemma
   (pre: Bytes → τ → Prop) [BytesCompatible pre] (x: SigInput) (tr: τ):
   isWellFormed pre x tr = (
-    pre x.x_pk tr ∧
-    pre x.y_pk tr
+    pre x.xPk tr ∧
+    pre x.yPk tr
   )
 
 grind_pattern SigInput.isWellFormedLemma => isWellFormed pre x tr
 grind_pattern [grind_later] SigInput.isWellFormedLemma => isWellFormed pre x tr
 
 inductive SignedDHEvent where
-  | ClientInitiateEvent (x_pk: Bytes)
-  | ServerFinishEvent (x_pk: Bytes) (y_pk: Bytes) (k_s: Bytes)
-  | ClientFinishEvent (server: Principal) (x_pk: Bytes) (y_pk: Bytes) (k_c: Bytes)
+  | ClientInitiateEvent (client: Participant) (xPk: Bytes)
+  | ServerFinishEvent (server: Participant) (xPk: Bytes) (yPk: Bytes) (kS: Bytes)
+  | ClientFinishEvent (client server: Participant) (xPk: Bytes) (yPk: Bytes) (kC: Bytes)
 
-instance : ParseableSerializeable SignedDHEvent := sorry
+def ClientEphemeralStateCompromised
+  [ExecTraceTypes]
+  [ExecTraceTypes.Has (PersistentLocalState.Compromise.ExecEntryT ClientInitiateState)]
+  [ExecTraceTypes.Has (PersistentLocalState.Compromise.ExecEntryT ClientFinishState)]
+  (me: Participant) (xPk: Bytes)
+  (tr: ExecTrace)
+  : Prop
+:=
+  (∃ xSk, PersistentLocalState.LocalStateCompromised me ({xPk, xSk}: ClientInitiateState) tr) ∨
+  (∃ kC, PersistentLocalState.LocalStateCompromised me ({xPk, kC}: ClientFinishState) tr)
 
--- setup
+theorem ClientEphemeralStateCompromised_le
+  [ExecTraceTypes]
+  [ExecTraceTypes.Has (PersistentLocalState.Compromise.ExecEntryT ClientInitiateState)]
+  [ExecTraceTypes.Has (PersistentLocalState.Compromise.ExecEntryT ClientFinishState)]
+  (me: Participant) (xPk: Bytes)
+  (tr1 tr2: ExecTrace)
+  : tr1 ≤ tr2 →
+    ClientEphemeralStateCompromised me xPk tr1 →
+    ClientEphemeralStateCompromised me xPk tr2
+:= by
+  simp only [ClientEphemeralStateCompromised]
+  grind
 
-def _root_.DY.Trace.prefix (tr: Trace α) (i: Nat): Trace α := sorry
-axiom prefix_le (tr: Trace α) (i: Nat): (tr.prefix i) ≤ tr
-grind_pattern prefix_le => tr.prefix i
+grind_pattern ClientEphemeralStateCompromised_le => tr1 ≤ tr2, ClientEphemeralStateCompromised me xPk tr1
 
-axiom event_logged_at (who: Principal) (ev: SignedDHEvent) (i: Nat) (tr: ProofTrace): Prop
-abbrev event_logged (who: Principal) (ev: SignedDHEvent) (tr: ProofTrace) :=
-  ∃ i, event_logged_at who ev i tr
+def client_label
+  [ExecTraceTypes]
+  [ExecTraceTypes.Has (PersistentLocalState.Compromise.ExecEntryT ClientInitiateState)]
+  [ExecTraceTypes.Has (PersistentLocalState.Compromise.ExecEntryT ClientFinishState)]
+  (me: Participant) (xPk: Bytes)
+  : Label
+where
+  isCorrupt tr := ClientEphemeralStateCompromised me xPk tr
 
-@[grind→, grind_later→]
-axiom event_logged_at_later (who: Principal) (ev: SignedDHEvent) (i: Nat) (tr1 tr2: ProofTrace): tr1 ≤ tr2 → event_logged_at who ev i tr1 → event_logged_at who ev i tr2
+def ServerEphemeralStateCompromised
+  [ExecTraceTypes]
+  [ExecTraceTypes.Has (PersistentLocalState.Compromise.ExecEntryT ServerFinishState)]
+  (me: Participant) (yPk: Bytes)
+  (tr: ExecTrace)
+  : Prop
+:=
+  (∃ kS, PersistentLocalState.LocalStateCompromised me ({yPk, kS}: ServerFinishState) tr)
 
+theorem ServerEphemeralStateCompromised_le
+  [ExecTraceTypes]
+  [ExecTraceTypes.Has (PersistentLocalState.Compromise.ExecEntryT ServerFinishState)]
+  (me: Participant) (yPk: Bytes)
+  (tr1 tr2: ExecTrace)
+  : tr1 ≤ tr2 →
+    ServerEphemeralStateCompromised me yPk tr1 →
+    ServerEphemeralStateCompromised me yPk tr2
+:= by
+  simp only [ServerEphemeralStateCompromised]
+  grind
 
-def gen_rand (len: Nat) : Traceful Bytes := sorry
-def send_message (b:Bytes) : Traceful Nat := sorry
-def receive_message (ts: Nat): Traceful Bytes := sorry
-def new_sid (me: Principal): Traceful Nat := sorry
-def set_client_state (me: Principal) (sid: Nat) (st: ClientState): Traceful Unit := sorry
-def get_client_state (me: Principal) (sid: Nat): Traceful ClientState  := sorry
-def set_server_state (me: Principal) (sid: Nat) (st: ServerState): Traceful Unit := sorry
-def get_server_state (me: Principal) (sid: Nat): Traceful ServerState  := sorry
-def get_public_key (who: Principal): Traceful Bytes := sorry
-def get_private_key (who: Principal): Traceful Bytes := sorry
-def log_event (who: Principal) (ev: SignedDHEvent): Traceful Unit := sorry
+grind_pattern ServerEphemeralStateCompromised_le => tr1 ≤ tr2, ServerEphemeralStateCompromised me yPk tr1
 
--- invariants
-
-instance: Inhabited Label where
-  default := Label.secret
-
-opaque client_label (me: Principal): Label
-opaque server_label (me: Principal): Label
-opaque long_term_label (me: Principal): Label
-
+def server_label
+  [ExecTraceTypes]
+  [ExecTraceTypes.Has (PersistentLocalState.Compromise.ExecEntryT ServerFinishState)]
+  (me: Participant) (yPk: Bytes)
+  : Label
+where
+  isCorrupt tr := ServerEphemeralStateCompromised me yPk tr
 
 structure LongTermKeyUsage where
-  principal: Principal
+  principal: Participant
 
 noncomputable
-instance : ParseableSerializeable LongTermKeyUsage := comparseExists
+instance : ParseableSerializeable LongTermKeyUsage := comparseMetaProgramExists
 
 @[grind]
 noncomputable
-def mk_long_term_usage (me: Principal): Usage := {
+def mk_long_term_usage (me: Participant): Usage := {
   type := "SigKey",
   tag := "SignedDH",
   data := serialize ({ principal := me }: LongTermKeyUsage)
@@ -261,58 +207,129 @@ theorem mk_long_term_usage_inj:
     simp [Function.Injective, mk_long_term_usage]
     grind
 
-instance: Signature.SignPred where
+
+instance SignedDHSignPred
+  [BytesFunctor.Has DiffieHellman.SubF]
+  [BytesFunctor.Has Hash.SubF]
+  [TraceTypes]
+  [ExecTraceTypes.Has (ProtocolEvent.ExecEntryT SignedDHEvent)]
+  [ExecTraceTypes.Has (PersistentLocalState.Compromise.ExecEntryT ServerFinishState)]
+  : Signature.SignPred
+where
   pred skUsg vk msg tr :=
     ∃ server, skUsg = mk_long_term_usage server ∧ (
       match parse msg with
       | none => False
       | some (msg: SigInput) => (
-        ∃ y_sk,
-          msg.y_pk = DiffieHellman.dh_pk y_sk ∧
-          y_sk.label tr = server_label server ∧
-          event_logged server (.ServerFinishEvent msg.x_pk msg.y_pk (Hash.hash (DiffieHellman.dh msg.x_pk y_sk))) tr
+        ∃ ySk,
+          msg.yPk = DiffieHellman.dh_pk ySk ∧
+          ySk.label tr = server_label server msg.yPk ∧
+          tr.erase.EventLogged (SignedDHEvent.ServerFinishEvent server msg.xPk msg.yPk (Hash.hash (DiffieHellman.dh msg.xPk ySk)))
       )
     )
 
-instance [BytesInvariants] [BytesInvariants.Has DiffieHellman.DhPk.invariants]: Signature.SignPredProof where
+instance
+  [BytesFunctor.Has DiffieHellman.SubF]
+  [BytesFunctor.Has Hash.SubF]
+  [TraceTypes]
+  [ExecTraceTypes.Has (ProtocolEvent.ExecEntryT SignedDHEvent)]
+  [ExecTraceTypes.Has (PersistentLocalState.Compromise.ExecEntryT ServerFinishState)]
+  [BytesInvariants]
+  [BytesInvariants.Has DiffieHellman.DhPk.invariants]
+  : Signature.SignPredProof
+where
   pred_later := by
     intro _ _ _ _ _ _ _ _ _ _ _
     intro ⟨ server, h ⟩
     exists server
     grind [DiffieHellman.dh_pk.WellFormed]
 
+section
+
+variable [TraceTypes]
 variable [BytesInvariants]
 variable [BytesInvariantsProofs]
-variable [BytesInvariants.Has Hash.invariants]
-variable [BytesInvariants.Has DiffieHellman.invariants]
-variable [BytesInvariants.Has Signature.invariants]
 
-def client_state_inv (me: Principal) (sid: Nat) (st: ClientState) (tr: ProofTrace) :=
-  match st with
-  | .ClientInitiateState x_sk =>
-    x_sk.Invariant tr ∧
-    x_sk.label tr = client_label me ∧
-    True -- usage
-  | .ClientFinishState k_c =>
-    k_c.Invariant tr ∧
-    (k_c.label tr).canFlow (client_label me) tr
+instance ClientInitiateStateInv
+  [BytesFunctor.Has DiffieHellman.SubF]
+  [ExecTraceTypes.Has (PersistentLocalState.CompromisableState.ExecEntryT ClientInitiateState)]
+  [ExecTraceTypes.Has (PersistentLocalState.CompromisableState.ExecEntryT ClientFinishState)]
+  : PersistentLocalState.CompromisableLocalStateInv ClientInitiateState
+where
+  invariant me st tr :=
+    let { xPk, xSk } := st
+    xPk = DiffieHellman.dh_pk xSk ∧
+    xPk.Publishable tr ∧
+    xSk.Invariant tr ∧
+    xSk.label tr = client_label me xPk
+  invariant_later := by grind
+  invariant_implies_KnowableBy participant state tr := by
+    have: (client_label participant state.xPk).canFlow (PersistentLocalState.label participant state) tr.erase := by
+      cases state
+      simp [Label.canFlow, client_label, ClientEphemeralStateCompromised]
+      grind
+    grind [canFlowTrans]
 
-@[grind→, grind_later→]
-theorem client_state_inv_later
-  (me: Principal) (sid: Nat) (st: ClientState) (tr1 tr2: ProofTrace):
-  tr1 ≤ tr2 → client_state_inv me sid st tr1 → client_state_inv me sid st tr2
-  := by
-    unfold client_state_inv
-    grind
+-- for monotonicity
+theorem ClientInitiateStateInv_imp_Invariant
+  [BytesFunctor.Has DiffieHellman.SubF]
+  [ExecTraceTypes.Has (PersistentLocalState.CompromisableState.ExecEntryT ClientInitiateState)]
+  [ExecTraceTypes.Has (PersistentLocalState.CompromisableState.ExecEntryT ClientFinishState)]
+  (participant: Participant) (st: ClientInitiateState)
+  : PersistentLocalState.LocalStateInv.invariant participant st tr → (
+      st.xSk.Invariant tr ∧
+      st.xPk.Invariant tr
+    )
+:= by
+  simp [PersistentLocalState.LocalStateInv.invariant]
+  grind
 
-def server_state_inv (me: Principal) (sid: Nat)(st: ServerState) (tr: ProofTrace) :=
-  match st with
-  | .ServerFinishState k_s =>
-    k_s.Invariant tr ∧
-    (k_s.label tr).canFlow (server_label me) tr
+grind_pattern [grind_later] ClientInitiateStateInv_imp_Invariant => PersistentLocalState.LocalStateInv.invariant participant st tr
 
-instance (sk: Bytes):
-  HoareTriplePure
+instance ClientFinishStateInv
+  [ExecTraceTypes.Has (PersistentLocalState.CompromisableState.ExecEntryT ClientInitiateState)]
+  [ExecTraceTypes.Has (PersistentLocalState.CompromisableState.ExecEntryT ClientFinishState)]
+  : PersistentLocalState.CompromisableLocalStateInv ClientFinishState
+where
+  invariant me st tr :=
+    let { xPk, kC } := st
+    xPk.Publishable tr ∧
+    kC.Invariant tr ∧
+    (kC.label tr).canFlow (client_label me xPk) tr.erase
+  invariant_later := by grind
+  invariant_implies_KnowableBy participant state tr := by
+    have: (client_label participant state.xPk).canFlow (PersistentLocalState.label participant state) tr.erase := by
+      cases state
+      simp [Label.canFlow, client_label, ClientEphemeralStateCompromised]
+      grind
+    grind [canFlowTrans]
+
+instance ServerFinishStateInv
+  [ExecTraceTypes.Has (PersistentLocalState.CompromisableState.ExecEntryT ServerFinishState)]
+  : PersistentLocalState.CompromisableLocalStateInv ServerFinishState
+where
+  invariant me st tr :=
+    let { yPk, kS } := st
+    yPk.Publishable tr ∧
+    kS.Invariant tr ∧
+    (kS.label tr).canFlow (server_label me yPk) tr.erase
+  invariant_later := by grind
+  invariant_implies_KnowableBy participant state tr := by
+    have: (server_label participant state.yPk).canFlow (PersistentLocalState.label participant state) tr.erase := by
+      cases state
+      simp [Label.canFlow, server_label, ServerEphemeralStateCompromised]
+      grind
+    grind [canFlowTrans]
+
+end
+
+instance
+  [TraceTypes]
+  [BytesInvariants]
+  [BytesFunctor.Has DiffieHellman.SubF]
+  [BytesInvariants.Has DiffieHellman.invariants]
+  (sk: Bytes)
+  : HoareTriplePure
     (DiffieHellman.dh_pk sk)
     (fun tr => sk.Invariant tr)
     (fun res tr =>
@@ -324,8 +341,13 @@ instance (sk: Bytes):
     pf := by
       grind [DiffieHellman.dh_pk.Invariant, DiffieHellman.dh_pk.label]
 
-instance (pk sk: Bytes):
-  HoareTriplePure
+instance
+  [TraceTypes]
+  [BytesInvariants]
+  [BytesFunctor.Has DiffieHellman.SubF]
+  [BytesInvariants.Has DiffieHellman.invariants]
+  (pk sk: Bytes)
+  : HoareTriplePure
     (DiffieHellman.dh pk sk)
     (fun tr =>
       sk.Invariant tr ∧
@@ -341,8 +363,14 @@ instance (pk sk: Bytes):
     pf := by
       grind [DiffieHellman.dh.Invariant, DiffieHellman.dh.label]
 
-instance (sk: Bytes):
-  HoareTriplePure
+instance
+  [TraceTypes]
+  [BytesInvariants]
+  [BytesFunctor.Has Signature.SubF]
+  [Signature.SignPred]
+  [BytesInvariants.Has Signature.invariants]
+  (sk: Bytes)
+  : HoareTriplePure
     (Signature.vk sk)
     (fun tr =>
       sk.Invariant tr
@@ -356,7 +384,10 @@ instance (sk: Bytes):
     pf := by
       grind [Signature.vk.Invariant, Signature.vk.label]
 
-instance (sk nonce msg: Bytes): HasGhostArgumentType (Signature.sign sk nonce msg) Usage
+instance
+  [BytesFunctor.Has Signature.SubF]
+  (sk nonce msg: Bytes)
+  : HasGhostArgumentType (Signature.sign sk nonce msg) Usage
 where
   dummy := ()
 
@@ -374,18 +405,29 @@ def signMetaprog: GhostParameterFinder where
 
     let usg_mvar: Lean.Expr := .mvar mvar
     let tr_mvar ← Lean.Meta.mkFreshExprMVar (some (← Lean.Meta.mkAppOptM ``ProofTrace #[none]))
-    let hasUsageToUnify ← Lean.Meta.mkAppOptM ``Bytes.HasUsage #[none, none, none, sk_mvar, usg_mvar, tr_mvar]
+    let hasUsageToUnify ← Lean.Meta.mkAppOptM ``Bytes.HasUsage #[none, none, none, none, sk_mvar, usg_mvar, tr_mvar]
     trace[Step] "gonna find {hasUsageToUnify} in assumptions"
     let .mvar hasUsageMvar ← Lean.Meta.mkFreshExprMVar hasUsageToUnify
       | throwError ""
-    hasUsageMvar.assumption
+    unless ← hasUsageMvar.assumptionCore do
+      throwError "Cannot find `sk.HasUsage _ _` in the context, please supply usage manually using `with ⟨ ... ⟩`"
+    pure ()
 
-instance (sk nonce msg: Bytes): HasGhostMetaprogram (Signature.sign sk nonce msg) signMetaprog
+instance
+  [BytesFunctor.Has Signature.SubF]
+  (sk nonce msg: Bytes)
+  : HasGhostMetaprogram (Signature.sign sk nonce msg) signMetaprog
 where
   dummy := ()
 
-instance (sk nonce msg: Bytes) (skUsg: Usage):
-  HoareTriplePureGhost
+instance
+  [TraceTypes]
+  [BytesInvariants]
+  [BytesFunctor.Has Signature.SubF]
+  [Signature.SignPred]
+  [BytesInvariants.Has Signature.invariants]
+  (sk nonce msg: Bytes) (skUsg: Usage)
+  : HoareTriplePureGhost
     (Signature.sign sk nonce msg)
     (skUsg)
     (fun tr =>
@@ -394,13 +436,13 @@ instance (sk nonce msg: Bytes) (skUsg: Usage):
       msg.Invariant tr ∧
       sk.HasUsage skUsg tr ∧
       --nonce `has_usage tr` SigNonce /\
-      (sk.label tr).canFlow (nonce.label tr) tr ∧
+      (sk.label tr).canFlow (nonce.label tr) tr.erase ∧
       (
         (
           skUsg.type = "SigKey" ∧
           Signature.SignPred.pred skUsg (Signature.vk sk) msg tr
         ) ∨ (
-          (sk.label tr).canFlow Label.pub tr
+          (sk.label tr).canFlow Label.pub tr.erase
         )
       )
     )
@@ -415,7 +457,9 @@ instance (sk nonce msg: Bytes) (skUsg: Usage):
       apply Signature.sign.Invariant sk nonce msg skUsg
       grind
 
-instance (vkey msg sig: Bytes): HasGhostArgumentType (Signature.verify vkey msg sig) Usage
+instance
+  [BytesFunctor.Has Signature.SubF]
+  (vkey msg sig: Bytes): HasGhostArgumentType (Signature.verify vkey msg sig) Usage
 where
   dummy := ()
 
@@ -433,18 +477,27 @@ def verifyMetaprog: GhostParameterFinder where
 
     let usg_mvar: Lean.Expr := .mvar mvar
     let tr_mvar ← Lean.Meta.mkFreshExprMVar (some (← Lean.Meta.mkAppOptM ``ProofTrace #[none]))
-    let hasUsageToUnify ← Lean.Meta.mkAppOptM ``Bytes.SignkeyHasUsage #[none, none, none, vkey_mvar, usg_mvar, tr_mvar]
+    let hasUsageToUnify ← Lean.Meta.mkAppOptM ``Bytes.SignkeyHasUsage #[none, none, none, none, vkey_mvar, usg_mvar, tr_mvar]
     trace[Step] "gonna find {hasUsageToUnify} in assumptions"
     let .mvar hasUsageMvar ← Lean.Meta.mkFreshExprMVar hasUsageToUnify
       | throwError ""
-    hasUsageMvar.assumption
+    unless ← hasUsageMvar.assumptionCore do
+      throwError "Cannot find `vk.SignkeyHasUsage _ _` in the context, please supply usage manually using `with ⟨ ... ⟩`"
 
-instance (vkey msg sig: Bytes): HasGhostMetaprogram (Signature.verify vkey msg sig) verifyMetaprog
+instance
+  [BytesFunctor.Has Signature.SubF]
+  (vkey msg sig: Bytes): HasGhostMetaprogram (Signature.verify vkey msg sig) verifyMetaprog
 where
   dummy := ()
 
-instance (vkey msg sig: Bytes) (skUsg: Usage):
-  HoareTriplePureGhost
+instance
+  [TraceTypes]
+  [BytesInvariants]
+  [BytesFunctor.Has Signature.SubF]
+  [Signature.SignPred]
+  [BytesInvariants.Has Signature.invariants]
+  (vkey msg sig: Bytes) (skUsg: Usage)
+  : HoareTriplePureGhost
     (Signature.verify vkey msg sig)
     (skUsg: Usage)
     (fun tr =>
@@ -459,7 +512,7 @@ instance (vkey msg sig: Bytes) (skUsg: Usage):
           skUsg.type = "SigKey" →
           Signature.SignPred.pred skUsg vkey msg tr
         ) ∨ (
-          (vkey.signkeyLabel tr).canFlow Label.pub tr
+          (vkey.signkeyLabel tr).canFlow Label.pub tr.erase
         )
       )
     )
@@ -470,8 +523,13 @@ instance (vkey msg sig: Bytes) (skUsg: Usage):
       apply Signature.verify.Invariant vkey msg sig skUsg <;>
       grind
 
-instance (b: Bytes):
-  HoareTriplePure
+instance
+  [TraceTypes]
+  [BytesInvariants]
+  [BytesFunctor.Has Hash.SubF]
+  [BytesInvariants.Has Hash.invariants]
+  (b: Bytes)
+  : HoareTriplePure
     (Hash.hash b)
     (fun tr => b.Invariant tr)
     (fun res tr =>
@@ -482,383 +540,314 @@ instance (b: Bytes):
     pf := by
       simp
 
-instance: HasGhostArgumentType (gen_rand len) Label
+section
+
+variable [TraceTypes]
+variable [BytesInvariants]
+variable [BytesInvariantsProofs]
+
+instance [BytesFunctor.Has Signature.SubF]: LongTermKeys.ExecConfig "SignedDH" Signature.vk where
+
+@[grind]
+noncomputable
+instance
+  [BytesFunctor.Has Signature.SubF] [Signature.SignPred] [BytesInvariants.Has Signature.invariants]
+  [ExecTraceTypes.Has <| LongTermKeys.ExecEntryT "SignedDH"]
+  : LongTermKeys.ProofConfig "SignedDH" mk_long_term_usage
 where
-  dummy := ()
+  IsLongTermPublicKey who vk tr :=
+    vk.Publishable tr ∧
+    vk.signkeyLabel tr = LongTermKeys.label "SignedDH" who vk ∧
+    vk.SignkeyHasUsage (mk_long_term_usage who) tr
 
-instance:
-  HoareTripleGhost
-    (gen_rand len)
-    lab
-    (fun _ => True)
-    (fun b tr =>
-      b.Invariant tr ∧
-      b.label tr = lab
-      -- usage, length
+  IsLongTermPublicKey_implied := by
+    simp_all [Bytes.Publishable]
+    grind
+
+instance SignedDHEventInv
+  [BytesFunctor]
+  [BytesFunctor.Has Signature.SubF]
+  [BytesFunctor.Has DiffieHellman.SubF]
+  [TraceTypes]
+  [ExecTraceTypes.Has (PersistentLocalState.Compromise.ExecEntryT ClientInitiateState)]
+  [ExecTraceTypes.Has (PersistentLocalState.Compromise.ExecEntryT ClientFinishState)]
+  [ExecTraceTypes.Has (PersistentLocalState.Compromise.ExecEntryT ServerFinishState)]
+  [ExecTraceTypes.Has (LongTermKeys.ExecEntryT "SignedDH")]
+  [BytesInvariants]
+  [ExecTraceTypes.Has (ProtocolEvent.ExecEntryT SignedDHEvent)]
+  : ProtocolEvent.EventInv (SignedDHEvent)
+where
+  invariant tr ev :=
+    match ev with
+    | SignedDHEvent.ClientInitiateEvent client xPk => (
+      xPk.Invariant tr ∧
+      xPk.dhSkLabel tr = client_label client xPk
     )
-  where
-    pf := sorry
-
-instance:
-  HoareTriple
-    (send_message b)
-    (fun tr => b.Publishable tr)
-    (fun _ _ => True)
-  where
-    pf := sorry
-
-instance:
-  HoareTriple
-    (receive_message ts)
-    (fun _ => True)
-    (fun b tr => b.Publishable tr)
-  where
-    pf := sorry
-
-instance:
-  HoareTriple
-    (new_sid me)
-    (fun _ => True)
-    (fun _ _ => True)
-  where
-    pf := sorry
-
-instance:
-  HoareTriple
-    (set_client_state me sid st)
-    (fun tr => client_state_inv me sid st tr)
-    (fun _ _ => True)
-  where
-    pf := sorry
-
-instance:
-  HoareTriple
-    (get_client_state me sid)
-    (fun _ => True)
-    (fun st tr => client_state_inv me sid st tr)
-  where
-    pf := sorry
-
-instance:
-  HoareTriple
-    (set_server_state me sid st)
-    (fun tr => server_state_inv me sid st tr)
-    (fun _ _ => True)
-  where
-    pf := sorry
-
-instance:
-  HoareTriple
-    (get_server_state me sid)
-    (fun _ => True)
-    (fun st tr => server_state_inv me sid st tr)
-  where
-    pf := sorry
-
-instance:
-  HoareTriple
-    (get_public_key who)
-    (fun _ => True)
-    (fun vk tr =>
-      vk.Invariant tr ∧
-      vk.signkeyLabel tr = long_term_label who ∧
-      vk.SignkeyHasUsage (mk_long_term_usage who) tr
+    | SignedDHEvent.ServerFinishEvent server xPk yPk kS => (
+      kS.Invariant tr ∧
+      xPk.Invariant tr ∧
+      kS.label tr = (server_label server yPk).join (xPk.dhSkLabel tr)
     )
-  where
-    pf := sorry
-
-instance:
-  HoareTriple
-    (get_private_key who)
-    (fun _ => True)
-    (fun sk tr =>
-      sk.Invariant tr ∧
-      sk.label tr = long_term_label who ∧
-      sk.HasUsage (mk_long_term_usage who) tr
+    | SignedDHEvent.ClientFinishEvent client server xPk yPk kC => (
+      (
+        tr.erase.EventLogged (SignedDHEvent.ServerFinishEvent server xPk yPk kC) ∧
+        kC.Invariant tr ∧
+        kC.label tr = (client_label client xPk).join (server_label server yPk)
+      ) ∨ (∃ spk, (LongTermKeys.label "SignedDH" server spk).isCorrupt tr.erase)
     )
-  where
-    pf := sorry
 
-def event_pred (me: Principal) (ev: SignedDHEvent) (tr: ProofTrace) :=
-  match ev with
-  | .ClientInitiateEvent x_pk => (
-    x_pk.Invariant tr ∧
-    x_pk.dhSkLabel tr = client_label me
-  )
-  | .ServerFinishEvent x_pk _y_pk k_s => (
-    k_s.Invariant tr ∧
-    x_pk.Invariant tr ∧
-    k_s.label tr = (server_label me).join (x_pk.dhSkLabel tr)
-  )
-  | .ClientFinishEvent server x_pk y_pk k_c => (
-    (
-      event_logged server (.ServerFinishEvent x_pk y_pk k_c) tr ∧
-      k_c.Invariant tr ∧
-      k_c.label tr = (client_label me).join (server_label server)
-    ) ∨ (long_term_label server).isCorrupt tr
-  )
-
-instance:
-  HoareTriple
-    (log_event who ev)
-    (fun tr => event_pred who ev tr)
-    (fun () tr => event_logged who ev tr)
-  where
-    pf := sorry
-
-@[grind→]
-axiom event_logged_at_implies_event_pred
-  (who: Principal) (ev: SignedDHEvent) (i: Nat) (tr: ProofTrace):
-    event_logged_at who ev i tr →
-    tr.invariant →
-    event_pred who ev (tr.prefix i)
-
--- signed dh
+end
 
 namespace SignedDH
 
-def client_initiate (me: Principal): Traceful (Nat × Nat) := do
-  let x_sk ← gen_rand 32
-  let x_pk := DiffieHellman.dh_pk x_sk
+section Specification
 
-  log_event me (.ClientInitiateEvent x_pk)
-  let sid ← new_sid me
-  set_client_state me sid (.ClientInitiateState x_sk)
-  let msg_ts ← send_message (serialize ({ x_pk } : ClientMessage))
-  pure (sid, msg_ts)
+variable [BytesFunctor.Has Random.SubF]
+variable [BytesFunctor.Has Hash.SubF]
+variable [BytesFunctor.Has DiffieHellman.SubF]
+variable [BytesFunctor.Has Signature.SubF]
+
+variable [ExecTraceTypes]
+variable [ExecTraceTypes.Has Network.ExecEntryT]
+variable [ExecTraceTypes.Has Random.ExecEntryT]
+variable [ExecTraceTypes.Has (ProtocolEvent.ExecEntryT SignedDHEvent)]
+variable [ExecTraceTypes.Has (LongTermKeys.ExecEntryT "SignedDH")]
+
+variable [ExecTraceTypes.Has (PersistentLocalState.CompromisableState.ExecEntryT ClientInitiateState)]
+variable [ExecTraceTypes.Has (PersistentLocalState.CompromisableState.ExecEntryT ClientFinishState)]
+variable [ExecTraceTypes.Has (PersistentLocalState.CompromisableState.ExecEntryT ServerFinishState)]
 
 noncomputable
-def server_receive (me: Principal) (msg_ts: Nat) : Traceful (Nat × Nat) := do
-  let msg_bytes ← receive_message msg_ts
+def client_initiate (me: Participant): Traceful (Nat × Nat) := do
+  let xSk ← Random.genRand 32
+  let xPk := DiffieHellman.dh_pk xSk
+
+  ProtocolEvent.logEvent (SignedDHEvent.ClientInitiateEvent me xPk)
+  let st_ts ← PersistentLocalState.storeLocalState me ({ xPk, xSk }: ClientInitiateState)
+  let msg_ts ← Network.sendMessage (serialize ({ xPk } : ClientMessage))
+  pure (st_ts, msg_ts)
+
+noncomputable
+def server_receive (me: Participant) (sk_ts: Nat) (msg_ts: Nat): Traceful (Nat × Nat) := do
+  let msg_bytes ← Network.receiveMessage msg_ts
   let msg: ClientMessage ← parse msg_bytes
-  let x_pk := msg.x_pk
-  let my_sig_key ← get_private_key me
+  let xPk := msg.xPk
+  let my_sig_key ← LongTermKeys.getPrivateKey "SignedDH" me sk_ts
 
-  let y_sk ← gen_rand 32
-  let y_pk := DiffieHellman.dh_pk y_sk
-  let k_s := Hash.hash (DiffieHellman.dh x_pk y_sk)
-  let sig_nonce ← gen_rand 32
-  let sig := Signature.sign my_sig_key sig_nonce (serialize ({x_pk, y_pk}: SigInput))
+  let ySk ← Random.genRand 32
+  let yPk := DiffieHellman.dh_pk ySk
+  let kS := Hash.hash (DiffieHellman.dh xPk ySk)
+  let sig_nonce ← Random.genRand 32
+  let sig := Signature.sign my_sig_key sig_nonce (serialize ({xPk, yPk}: SigInput))
 
-  log_event me (.ServerFinishEvent x_pk y_pk k_s)
-  let sid ← new_sid me
-  set_server_state me sid (.ServerFinishState k_s)
-  let msg_ts ← send_message (serialize ({ y_pk, sig } : ServerMessage))
-  pure (sid, msg_ts)
+  ProtocolEvent.logEvent (SignedDHEvent.ServerFinishEvent me xPk yPk kS)
+  let st_ts ← PersistentLocalState.storeLocalState me ({ yPk, kS }: ServerFinishState)
+  let msg_ts ← Network.sendMessage (serialize ({ yPk, sig } : ServerMessage))
+  pure (st_ts, msg_ts)
 
 noncomputable
-def client_finish (me: Principal) (server: Principal) (msg_ts: Nat) (sid: Nat) : Traceful Unit := do
-  let msg_bytes ← receive_message msg_ts
+def client_finish (me: Participant) (server: Participant) (pk_ts: Nat) (msg_ts: Nat) (sid: Nat) : Traceful Unit := do
+  let msg_bytes ← Network.receiveMessage msg_ts
   let msg: ServerMessage ← parse msg_bytes
 
-  let my_state ← get_client_state me sid
-  let .ClientInitiateState x_sk := my_state
-    | OptionT.fail
+  let ({xPk, xSk}: ClientInitiateState) ← PersistentLocalState.getLocalState me sid
+  let server_vk ← LongTermKeys.getPublicKey "SignedDH" server pk_ts
 
-  let server_vk ← get_public_key server
+  guard (Signature.verify server_vk (serialize ({ xPk, yPk := msg.yPk }: SigInput)) msg.sig)
+  let kC := Hash.hash (DiffieHellman.dh msg.yPk xSk)
 
-  let x_pk := DiffieHellman.dh_pk x_sk
-  guard (Signature.verify server_vk (serialize ({ x_pk, y_pk := msg.y_pk }: SigInput)) msg.sig)
-  let k_c := Hash.hash (DiffieHellman.dh msg.y_pk x_sk)
+  ProtocolEvent.logEvent (SignedDHEvent.ClientFinishEvent me server xPk msg.yPk kC)
+  let _ ← PersistentLocalState.storeLocalState me ({ xPk, kC }: ClientFinishState)
 
-  log_event me (.ClientFinishEvent server x_pk msg.y_pk k_c)
-  set_client_state me sid (.ClientFinishState k_c)
+end Specification
 
-instance:
-  HoareTriple
-    (client_initiate me)
-    (fun _ => True)
-    (fun _ _ => True)
-where
-  pf := by
-    unfold client_initiate
-    step with ⟨ client_label me ⟩
-    step
-    step by grind [event_pred]
-    step
-    step by grind [client_state_inv]
-    step
-    step
-    grind
+section SecurityTheorems
 
-instance:
-  HoareTriple
-    (server_receive me msg_ts)
-    (fun _ => True)
-    (fun _ _ => True)
-where
-  pf := by
-    unfold server_receive
-    step
-    step
-    step_intro
-    step
-    step with ⟨ server_label me ⟩
-    step
-    hoist
-    step
-    step
-    step with ⟨ Label.secret ⟩
-    hoist
-    step_intro
-    -- for monotonicity TODO: how to infer Publishable automatically?
-    have h_sig_msg: sig_msg.Publishable tr := by grind
-    -- interesting stuff: we will prove things on `sig` later on,
-    -- because we need to log the event before
-    step_intro
-    step by grind [event_pred]
-    step_let sig with ⟨ mk_long_term_usage me ⟩ by
-      simp only [Signature.SignPred.pred]
-      grind
-    step
-    step by grind [server_state_inv]
-    step
-    step
-    grind
+variable [TraceInvariant] [BytesInvariants] [BytesInvariantsProofs]
+variable [BaseAttackerKnowledge] [AttackerKnowledge] [BaseAttackerKnowledgeTheorem] [AttackerKnowledgeTheorem]
 
-instance:
-  HoareTriple
-    (client_finish me server msg_ts sid)
-    (fun _ => True)
-    (fun _ _ => True)
-where
-  pf := by
-    unfold client_finish
-    step
-    step
-    step
-    split
-    case h_1 x_sk h_x_sk =>
-      -- this is useful to monotonize hypothesis
-      -- (probably best as a grind pattern on client_state_inv but well)
-      have h_x_sk': x_sk.Invariant tr := by grind [client_state_inv]
-      step
-      step
-      step with ⟨ mk_long_term_usage server ⟩
-      hoist
-      step
-      step
-      step by
-        simp_all [event_pred, Signature.SignPred.pred]
-        grind [event_pred, client_state_inv]
-      step by grind [client_state_inv]
-      grind
-    · step
-      grind
+variable [BytesFunctor.Has Signature.SubF]
+variable [BytesFunctor.Has DiffieHellman.SubF]
 
-theorem client_auth:
-  event_logged_at client (.ClientFinishEvent server x_pk y_pk k) time tr →
-  tr.invariant → (
+variable [TraceTypes.Has (ProtocolEvent.ProofEntryT SignedDHEvent)]
+variable [TraceTypes.Has (LongTermKeys.ProofEntryT "SignedDH")]
+
+variable [TraceTypes.Has (PersistentLocalState.CompromisableState.ProofEntryT ClientInitiateState)]
+variable [TraceTypes.Has (PersistentLocalState.CompromisableState.ProofEntryT ClientFinishState)]
+variable [TraceTypes.Has (PersistentLocalState.CompromisableState.ProofEntryT ServerFinishState)]
+
+variable [TraceInvariant.Has (ProtocolEvent.ProofEntryT SignedDHEvent)]
+
+
+theorem client_auth
+  (client server: Participant)
+  (xPk yPk k: Bytes)
+  (time: Nat)
+  (tr: ProofTrace):
+  tr.erase.EventLoggedAt (SignedDHEvent.ClientFinishEvent client server xPk yPk k) time →
+  tr.Invariant → -- reachable
+  (
     let tr_before := tr.prefix time
-    event_logged server (.ServerFinishEvent x_pk y_pk k) tr_before  ∨
-    (long_term_label server).isCorrupt tr_before
+    tr_before.erase.EventLogged (SignedDHEvent.ServerFinishEvent server xPk yPk k) ∨
+    (∃ spk, LongTermKeys.LongTermKeyCompromised "SignedDH" server spk tr_before.erase)
   )
-  := by
-    intro h_ev h_trinv
-    have := event_logged_at_implies_event_pred _ _ _ _ h_ev h_trinv
-    simp [event_pred] at this
-    grind
+:= by
+  intro h_ev h_trinv
+  have := Trace.EventLoggedAt_imp_EventInv _ _ _ h_trinv h_ev
+  simp [ProtocolEvent.EventInv.invariant, LongTermKeys.label] at this
+  grind
 
-theorem client_secrecy:
-  k.Publishable tr → -- attacker_knows
-  event_logged_at client (.ClientFinishEvent server x_pk y_pk k) time tr →
-  tr.invariant → (
+theorem client_secrecy
+  (client server: Participant)
+  (xPk yPk k: Bytes)
+  (tr: ProofTrace):
+  k.AttackerKnows tr.erase →
+  tr.erase.EventLoggedAt (SignedDHEvent.ClientFinishEvent client server xPk yPk k) time →
+  tr.Invariant → -- reachable
+  (
     let tr_before := tr.prefix time
-    (long_term_label server).isCorrupt tr_before ∨
-    (client_label client).isCorrupt tr ∨
-    (server_label server).isCorrupt tr
+    (∃ spk, LongTermKeys.LongTermKeyCompromised "SignedDH" server spk tr_before.erase) ∨
+    ClientEphemeralStateCompromised client xPk tr.erase ∨
+    ServerEphemeralStateCompromised server yPk tr.erase
   )
   := by
     intro h_pub h_ev h_trinv
-    have h_ev := event_logged_at_implies_event_pred _ _ _ _ h_ev h_trinv
-    simp [event_pred] at h_ev
+    have := Trace.EventLoggedAt_imp_EventInv _ _ _ h_trinv h_ev
+    simp [ProtocolEvent.EventInv.invariant] at this
+    simp_all [client_label, server_label, LongTermKeys.label]
     grind
 
+end SecurityTheorems
 
 namespace TestGrindAnnot
 
--- Test for a more automatic feeling
-attribute [grind] event_pred
-attribute [grind] client_state_inv
-attribute [grind] server_state_inv
-attribute [grind] Signature.SignPred.pred
-attribute [grind] instSignPred
+variable [BytesFunctor.Has Random.SubF]
+variable [BytesFunctor.Has Hash.SubF]
+variable [BytesFunctor.Has DiffieHellman.SubF]
+variable [BytesFunctor.Has Signature.SubF]
 
-instance:
+variable [TraceInvariant]
+variable [BytesInvariants] [BytesInvariantsProofs]
+
+variable [TraceTypes.Has Network.ProofEntryT]
+variable [TraceTypes.Has Random.ProofEntryT]
+variable [TraceTypes.Has (ProtocolEvent.ProofEntryT SignedDHEvent)]
+variable [TraceTypes.Has <| LongTermKeys.ProofEntryT "SignedDH"]
+
+variable [TraceTypes.Has (PersistentLocalState.CompromisableState.ProofEntryT ClientInitiateState)]
+variable [TraceTypes.Has (PersistentLocalState.CompromisableState.ProofEntryT ClientFinishState)]
+variable [TraceTypes.Has (PersistentLocalState.CompromisableState.ProofEntryT ServerFinishState)]
+
+variable [BytesInvariants.Has DiffieHellman.invariants]
+variable [BytesInvariants.Has Hash.invariants]
+variable [BytesInvariants.Has Signature.invariants]
+variable [BytesInvariants.Has Random.invariants]
+
+variable [TraceInvariant.Has Network.ProofEntryT]
+variable [TraceInvariant.Has Random.ProofEntryT]
+variable [TraceInvariant.Has (ProtocolEvent.ProofEntryT SignedDHEvent)]
+variable [TraceInvariant.Has <| LongTermKeys.ProofEntryT "SignedDH"]
+
+variable [TraceInvariant.Has (PersistentLocalState.CompromisableState.ProofEntryT ClientInitiateState)]
+variable [TraceInvariant.Has (PersistentLocalState.CompromisableState.ProofEntryT ClientFinishState)]
+variable [TraceInvariant.Has (PersistentLocalState.CompromisableState.ProofEntryT ServerFinishState)]
+
+-- Test for a more automatic feeling
+attribute [grind] ProtocolEvent.EventInv.invariant
+attribute [grind] SignedDHEventInv
+attribute [grind] ClientInitiateStateInv
+attribute [grind] ClientFinishStateInv
+attribute [grind] ServerFinishStateInv
+attribute [grind] Signature.SignPred.pred
+attribute [grind] SignedDHSignPred
+attribute [grind] PersistentLocalState.LocalStateInv.invariant
+attribute [grind] PersistentLocalState.CompromisableLocalStateInv.toLocalStateInv
+attribute [grind] LongTermKeys.IsLongTermPublicKey
+attribute [grind] LongTermKeys.IsLongTermSecretKey
+
+@[instance]
+theorem client_initiate.spec:
   HoareTriple
     (client_initiate me)
     (fun _ => True)
     (fun _ _ => True)
-where
-  pf := by
-    unfold client_initiate
-    step with ⟨ client_label me ⟩
-    step
-    step
-    step
-    step
-    step
-    step
+:= by
+  apply HoareTriple.mk
+  unfold client_initiate
+  step with ⟨ fun xSk => client_label me (DiffieHellman.dh_pk xSk), Usage.nothing ⟩
+  step
+  step
+  step by
+    simp only [PersistentLocalState.LocalStateInv.invariant]
     grind
+  step
+  step
+  grind
 
-instance:
+@[instance]
+theorem server_receive.spec:
   HoareTriple
-    (server_receive me msg_ts)
+    (server_receive me sk_ts msg_ts)
     (fun _ => True)
     (fun _ _ => True)
-where
-  pf := by
-    unfold server_receive
-    step
-    step
-    step_intro
-    step
-    step with ⟨ server_label me ⟩
-    step
-    hoist
-    step
-    step
-    step with ⟨ Label.secret ⟩
-    hoist
-    step_intro
-    -- for monotonicity TODO: how to infer Publishable automatically?
-    have h_sig_msg: sig_msg.Publishable tr := by grind
-    -- interesting stuff: we will prove things on `sig` later on,
-    -- because we need to log the event before
-    step_intro
-    step
-    step_let sig
-    step
-    step
-    step
-    step
+:= by
+  apply HoareTriple.mk
+  unfold server_receive
+  step
+  step
+  step_intro
+  step
+  step with ⟨ fun ySk => server_label me (DiffieHellman.dh_pk ySk), Usage.nothing ⟩
+  step
+  hoist
+  step
+  step
+  step with ⟨ fun _ => Label.secret, Usage.nothing ⟩
+  hoist
+  step_intro
+  step_intro -- interesting stuff: we will prove things on `sig` later on, because we need to log the event before
+  step
+  step_let sig with ⟨ mk_long_term_usage me ⟩
+  step by
+    simp only [PersistentLocalState.LocalStateInv.invariant]
     grind
+  step by
+    have: sig_msg.Publishable tr := by grind -- TODO how to infer this automatically?
+    grind
+  step
+  grind
 
-instance:
+@[instance]
+theorem client_finish.spec:
   HoareTriple
-    (client_finish me server msg_ts sid)
+    (client_finish me server pk_ts msg_ts sid)
     (fun _ => True)
     (fun _ _ => True)
-where
-  pf := by
-    unfold client_finish
-    step
-    step
-    step
-    split
-    case h_1 x_sk h_x_sk =>
-      have h_x_sk': x_sk.Invariant tr := by grind [client_state_inv] -- TODO: grind_later pattern?
-      step
-      step
-      step
-      hoist
-      step
-      step
-      step
-      step
-      grind
-    · step
-      grind
+:= by
+  apply HoareTriple.mk
+  unfold client_finish
+  step
+  step
+  step
+  split
+  step
+  step with ⟨ mk_long_term_usage server ⟩ by
+    simp_all only [PersistentLocalState.LocalStateInv.invariant]
+    grind
+  hoist
+  step by
+    simp_all only [PersistentLocalState.LocalStateInv.invariant]
+    grind
+  step
+  step by
+    simp_all only [PersistentLocalState.LocalStateInv.invariant]
+    grind
+  step by
+    simp_all only [PersistentLocalState.LocalStateInv.invariant]
+    grind
+  step_intro
+  step
+  grind
 
 end TestGrindAnnot
 
@@ -866,10 +855,11 @@ end SignedDH
 
 end Test
 
-abbrev SubF.internal: (id: Fin 3) → (Type → Type)
+abbrev SubF.internal: (id: Fin 4) → (Type → Type)
   | 0 => Hash.SubF
   | 1 => Signature.SubF
   | 2 => DiffieHellman.SubF
+  | 3 => Random.SubF
 
 abbrev SubF := BytesFunctor.combine SubF.internal
 
@@ -877,10 +867,12 @@ instance: ∀ id, SubBytesFunctor (SubF.internal id)
   | 0 => inferInstance
   | 1 => inferInstance
   | 2 => inferInstance
+  | 3 => inferInstance
 
 instance: BytesFunctor.HasStep Hash.SubF SubF := inferInstanceAs (BytesFunctor.HasStep (SubF.internal 0) SubF)
 instance: BytesFunctor.HasStep Signature.SubF SubF := inferInstanceAs (BytesFunctor.HasStep (SubF.internal 1) SubF)
 instance: BytesFunctor.HasStep DiffieHellman.SubF SubF := inferInstanceAs (BytesFunctor.HasStep (SubF.internal 2) SubF)
+instance: BytesFunctor.HasStep Random.SubF SubF := inferInstanceAs (BytesFunctor.HasStep (SubF.internal 3) SubF)
 
 instance: BytesFunctor where
   BytesF := SubF
@@ -890,11 +882,13 @@ instance: BytesFunctor.Has SubF := inferInstanceAs (BytesFunctor.Has BytesF)
 example: BytesFunctor.Has Hash.SubF := inferInstance
 example: BytesFunctor.Has Signature.SubF := inferInstance
 example: BytesFunctor.Has DiffieHellman.SubF := inferInstance
+example: BytesFunctor.Has Random.SubF := inferInstance
 
 def SubF.length.internal [BytesFunctor]: ∀ id, Bytes.PartialLength (SubF.internal id)
   | 0 => Hash.SubF.length
   | 1 => Signature.SubF.length
   | 2 => DiffieHellman.SubF.length
+  | 3 => Random.SubF.length
 
 abbrev SubF.length [BytesFunctor]: Bytes.PartialLength SubF :=
   Bytes.PartialLength.combine SubF.length.internal
@@ -905,18 +899,21 @@ instance: BytesLength where
 instance: BytesLength.HasStep Hash.SubF.length SubF.length := inferInstanceAs (BytesLength.HasStep (SubF.length.internal 0) SubF.length)
 instance: BytesLength.HasStep Signature.SubF.length SubF.length := inferInstanceAs (BytesLength.HasStep (SubF.length.internal 1) SubF.length)
 instance: BytesLength.HasStep DiffieHellman.SubF.length SubF.length := inferInstanceAs (BytesLength.HasStep (SubF.length.internal 2) SubF.length)
+instance: BytesLength.HasStep Random.SubF.length SubF.length := inferInstanceAs (BytesLength.HasStep (SubF.length.internal 3) SubF.length)
 
 instance: BytesLength.Has SubF.length := inferInstanceAs (BytesLength.Has SubF.length)
 
 example: BytesLength.Has Hash.SubF.length := inferInstance
 example: BytesLength.Has Signature.SubF.length := inferInstance
 example: BytesLength.Has DiffieHellman.SubF.length := inferInstance
+example: BytesLength.Has Random.SubF.length := inferInstance
 
-def attackerKnowledge.internal (id: Fin 3): SubAttackerKnowledge (SubF.internal id) :=
+def attackerKnowledge.internal (id: Fin 4): SubAttackerKnowledge (SubF.internal id) :=
   match id with
   | 0 => Hash.attackerKnowledge
   | 1 => Signature.attackerKnowledge
   | 2 => DiffieHellman.attackerKnowledge
+  | 3 => Random.attackerKnowledge
 
 def attackerKnowledge: SubAttackerKnowledge SubF :=
   SubAttackerKnowledge.combine attackerKnowledge.internal
@@ -924,6 +921,7 @@ def attackerKnowledge: SubAttackerKnowledge SubF :=
 instance: AttackerKnowledge.HasStep Hash.attackerKnowledge attackerKnowledge := inferInstanceAs (AttackerKnowledge.HasStep (attackerKnowledge.internal 0) (SubAttackerKnowledge.combine attackerKnowledge.internal))
 instance: AttackerKnowledge.HasStep Signature.attackerKnowledge attackerKnowledge := inferInstanceAs (AttackerKnowledge.HasStep (attackerKnowledge.internal 1) (SubAttackerKnowledge.combine attackerKnowledge.internal))
 instance: AttackerKnowledge.HasStep DiffieHellman.attackerKnowledge attackerKnowledge := inferInstanceAs (AttackerKnowledge.HasStep (attackerKnowledge.internal 2) (SubAttackerKnowledge.combine attackerKnowledge.internal))
+instance: AttackerKnowledge.HasStep Random.attackerKnowledge attackerKnowledge := inferInstanceAs (AttackerKnowledge.HasStep (attackerKnowledge.internal 3) (SubAttackerKnowledge.combine attackerKnowledge.internal))
 
 instance: AttackerKnowledge where
   attackerKnowledge
@@ -933,11 +931,113 @@ instance: AttackerKnowledge.Has attackerKnowledge := inferInstanceAs (AttackerKn
 example: AttackerKnowledge.Has Hash.attackerKnowledge := inferInstance
 example: AttackerKnowledge.Has Signature.attackerKnowledge := inferInstance
 example: AttackerKnowledge.Has DiffieHellman.attackerKnowledge := inferInstance
+example: AttackerKnowledge.Has Random.attackerKnowledge := inferInstance
 
-def invariants.internal: (id: Fin 3) → Bytes.PartialInvariants (SubF.internal id)
+@[expose]
+public
+def ExecEntryT.internal: Fin 7 → Type
+  | 0 => Network.ExecEntryT
+  | 1 => Random.ExecEntryT
+  | 2 => ProtocolEvent.ExecEntryT Test.SignedDHEvent
+  | 3 => PersistentLocalState.CompromisableState.ExecEntryT Test.ClientInitiateState
+  | 4 => PersistentLocalState.CompromisableState.ExecEntryT Test.ClientFinishState
+  | 5 => PersistentLocalState.CompromisableState.ExecEntryT Test.ServerFinishState
+  | 6 => LongTermKeys.ExecEntryT "SignedDH"
+
+public
+abbrev ExecEntryT: Type :=
+  ExecTraceTypes.combine ExecEntryT.internal
+
+instance: ExecTraceTypes.HasStep Network.ExecEntryT ExecEntryT := inferInstanceAs (ExecTraceTypes.HasStep (ExecEntryT.internal 0) (ExecTraceTypes.combine ExecEntryT.internal))
+instance: ExecTraceTypes.HasStep Random.ExecEntryT ExecEntryT := inferInstanceAs (ExecTraceTypes.HasStep (ExecEntryT.internal 1) (ExecTraceTypes.combine ExecEntryT.internal))
+instance: ExecTraceTypes.HasStep (ProtocolEvent.ExecEntryT Test.SignedDHEvent) ExecEntryT := inferInstanceAs (ExecTraceTypes.HasStep (ExecEntryT.internal 2) (ExecTraceTypes.combine ExecEntryT.internal))
+instance: ExecTraceTypes.HasStep (PersistentLocalState.CompromisableState.ExecEntryT Test.ClientInitiateState) ExecEntryT := inferInstanceAs (ExecTraceTypes.HasStep (ExecEntryT.internal 3) (ExecTraceTypes.combine ExecEntryT.internal))
+instance: ExecTraceTypes.HasStep (PersistentLocalState.CompromisableState.ExecEntryT Test.ClientFinishState) ExecEntryT := inferInstanceAs (ExecTraceTypes.HasStep (ExecEntryT.internal 4) (ExecTraceTypes.combine ExecEntryT.internal))
+instance: ExecTraceTypes.HasStep (PersistentLocalState.CompromisableState.ExecEntryT Test.ServerFinishState) ExecEntryT := inferInstanceAs (ExecTraceTypes.HasStep (ExecEntryT.internal 5) (ExecTraceTypes.combine ExecEntryT.internal))
+instance: ExecTraceTypes.HasStep (LongTermKeys.ExecEntryT "SignedDH") ExecEntryT := inferInstanceAs (ExecTraceTypes.HasStep (ExecEntryT.internal 6) (ExecTraceTypes.combine ExecEntryT.internal))
+
+instance: ExecTraceTypes where
+  ExecT := ExecEntryT
+
+instance: ExecTraceTypes.Has ExecEntryT := inferInstanceAs (ExecTraceTypes.Has ExecTrace.Entry)
+
+example: ExecTraceTypes.Has Network.ExecEntryT := inferInstance
+example: ExecTraceTypes.Has Random.ExecEntryT := inferInstance
+example: ExecTraceTypes.Has (ProtocolEvent.ExecEntryT Test.SignedDHEvent) := inferInstance
+example: ExecTraceTypes.Has (PersistentLocalState.CompromisableState.ExecEntryT Test.ClientInitiateState) := inferInstance
+example: ExecTraceTypes.Has (PersistentLocalState.CompromisableState.ExecEntryT Test.ClientFinishState) := inferInstance
+example: ExecTraceTypes.Has (PersistentLocalState.CompromisableState.ExecEntryT Test.ServerFinishState) := inferInstance
+example: ExecTraceTypes.Has (LongTermKeys.ExecEntryT "SignedDH") := inferInstance
+
+public
+def baseAttackerKnowledge.internal: (id: Fin 7) → SubBaseAttackerKnowledge (ExecEntryT.internal id)
+  | 0 => Network.baseAttackerKnowledge
+  | 1 => Random.baseAttackerKnowledge
+  | 2 => ProtocolEvent.baseAttackerKnowledge Test.SignedDHEvent
+  | 3 => PersistentLocalState.CompromisableState.baseAttackerKnowledge Test.ClientInitiateState
+  | 4 => PersistentLocalState.CompromisableState.baseAttackerKnowledge Test.ClientFinishState
+  | 5 => PersistentLocalState.CompromisableState.baseAttackerKnowledge Test.ServerFinishState
+  | 6 => LongTermKeys.baseAttackerKnowledge "SignedDH"
+
+public
+def baseAttackerKnowledge: SubBaseAttackerKnowledge ExecEntryT :=
+  SubBaseAttackerKnowledge.combine baseAttackerKnowledge.internal
+
+instance: BaseAttackerKnowledge where
+  attackerKnows := baseAttackerKnowledge
+
+-- Has trace attacker knowledge?
+
+@[expose]
+public
+def ProofEntryT.internal: Fin 7 → Type
+  | 0 => Network.ProofEntryT
+  | 1 => Random.ProofEntryT
+  | 2 => ProtocolEvent.ProofEntryT Test.SignedDHEvent
+  | 3 => PersistentLocalState.CompromisableState.ProofEntryT Test.ClientInitiateState
+  | 4 => PersistentLocalState.CompromisableState.ProofEntryT Test.ClientFinishState
+  | 5 => PersistentLocalState.CompromisableState.ProofEntryT Test.ServerFinishState
+  | 6 => LongTermKeys.ProofEntryT "SignedDH"
+
+public
+abbrev ProofEntryT: Type :=
+  TraceTypes.combine ProofEntryT.internal
+
+public
+instance: ∀ id, ErasableProofEntry (ExecEntryT.internal id) (ProofEntryT.internal id)
+  | 0 | 1 | 2 | 3 | 4 | 5 | 6 => by dsimp only [ExecEntryT.internal, ProofEntryT.internal]; infer_instance
+
+public
+instance: ErasableProofEntry ExecEntryT ProofEntryT :=
+  (inferInstance: ErasableProofEntry (ExecTraceTypes.combine ExecEntryT.internal) (TraceTypes.combine ProofEntryT.internal))
+
+instance: TraceTypes.HasStep Network.ProofEntryT ProofEntryT := inferInstanceAs (TraceTypes.HasStep (ProofEntryT.internal 0) (TraceTypes.combine ProofEntryT.internal))
+instance: TraceTypes.HasStep Random.ProofEntryT ProofEntryT := inferInstanceAs (TraceTypes.HasStep (ProofEntryT.internal 1) (TraceTypes.combine ProofEntryT.internal))
+instance: TraceTypes.HasStep (ProtocolEvent.ProofEntryT Test.SignedDHEvent) ProofEntryT := inferInstanceAs (TraceTypes.HasStep (ProofEntryT.internal 2) (TraceTypes.combine ProofEntryT.internal))
+instance: TraceTypes.HasStep (PersistentLocalState.CompromisableState.ProofEntryT Test.ClientInitiateState) ProofEntryT := inferInstanceAs (TraceTypes.HasStep (ProofEntryT.internal 3) (TraceTypes.combine ProofEntryT.internal))
+instance: TraceTypes.HasStep (PersistentLocalState.CompromisableState.ProofEntryT Test.ClientFinishState) ProofEntryT := inferInstanceAs (TraceTypes.HasStep (ProofEntryT.internal 4) (TraceTypes.combine ProofEntryT.internal))
+instance: TraceTypes.HasStep (PersistentLocalState.CompromisableState.ProofEntryT Test.ServerFinishState) ProofEntryT := inferInstanceAs (TraceTypes.HasStep (ProofEntryT.internal 5) (TraceTypes.combine ProofEntryT.internal))
+instance: TraceTypes.HasStep (LongTermKeys.ProofEntryT "SignedDH") ProofEntryT := inferInstanceAs (TraceTypes.HasStep (ProofEntryT.internal 6) (TraceTypes.combine ProofEntryT.internal))
+
+instance: TraceTypes where
+  ProofT := ProofEntryT
+  tc := inferInstance
+
+instance: TraceTypes.Has ProofEntryT := inferInstanceAs (TraceTypes.Has ProofTrace.Entry)
+
+example: TraceTypes.Has Network.ProofEntryT := inferInstance
+example: TraceTypes.Has Random.ProofEntryT := inferInstance
+example: TraceTypes.Has (ProtocolEvent.ProofEntryT Test.SignedDHEvent) := inferInstance
+example: TraceTypes.Has (PersistentLocalState.CompromisableState.ProofEntryT Test.ClientInitiateState) := inferInstance
+example: TraceTypes.Has (PersistentLocalState.CompromisableState.ProofEntryT Test.ClientFinishState) := inferInstance
+example: TraceTypes.Has (PersistentLocalState.CompromisableState.ProofEntryT Test.ServerFinishState) := inferInstance
+example: TraceTypes.Has (LongTermKeys.ProofEntryT "SignedDH") := inferInstance
+
+def invariants.internal: (id: Fin 4) → Bytes.PartialInvariants (SubF.internal id)
   | 0 => Hash.invariants
   | 1 => Signature.invariants
   | 2 => DiffieHellman.invariants
+  | 3 => Random.invariants
 
 abbrev invariants: Bytes.PartialInvariants SubF :=
   Bytes.PartialInvariants.combine invariants.internal
@@ -945,6 +1045,7 @@ abbrev invariants: Bytes.PartialInvariants SubF :=
 instance [BytesInvariants]: BytesInvariants.HasStep Hash.invariants invariants := inferInstanceAs (BytesInvariants.HasStep (invariants.internal 0) invariants)
 instance [BytesInvariants]: BytesInvariants.HasStep Signature.invariants invariants := inferInstanceAs (BytesInvariants.HasStep (invariants.internal 1) invariants)
 instance [BytesInvariants]: BytesInvariants.HasStep DiffieHellman.invariants invariants := inferInstanceAs (BytesInvariants.HasStep (invariants.internal 2) invariants)
+instance [BytesInvariants]: BytesInvariants.HasStep Random.invariants invariants := inferInstanceAs (BytesInvariants.HasStep (invariants.internal 3) invariants)
 
 instance: BytesInvariants where
   invs := invariants
@@ -954,11 +1055,13 @@ instance: BytesInvariants.Has invariants := inferInstance
 example: BytesInvariants.Has Hash.invariants := inferInstance
 example: BytesInvariants.Has Signature.invariants := inferInstance
 example: BytesInvariants.Has DiffieHellman.invariants := inferInstance
+example: BytesInvariants.Has Random.invariants := inferInstance
 
-def invariantsProofs.internal: (id: Fin 3) → Bytes.PartialInvariantsProofs (invariants.internal id)
+def invariantsProofs.internal: (id: Fin 4) → Bytes.PartialInvariantsProofs (invariants.internal id)
   | 0 => Hash.invariantsProofs
   | 1 => Signature.invariantsProofs
   | 2 => DiffieHellman.invariantsProofs
+  | 3 => Random.invariantsProofs
 
 abbrev invariantsProofs: Bytes.PartialInvariantsProofs invariants :=
   Bytes.PartialInvariantsProofs.combine invariantsProofs.internal
@@ -966,10 +1069,63 @@ abbrev invariantsProofs: Bytes.PartialInvariantsProofs invariants :=
 instance: BytesInvariantsProofs where
   pfs := invariantsProofs
 
-instance: (id: Fin 3) → SubAttackerKnowledgeTheorem (attackerKnowledge.internal id)
+public
+noncomputable
+instance: ∀ id, SubTraceInvariant (ProofEntryT.internal id)
+  | 0 | 1 | 2 | 3 | 4 | 5 | 6 => by dsimp only [ProofEntryT.internal]; infer_instance
+
+public
+noncomputable
+instance: SubTraceInvariant ProofEntryT :=
+  (inferInstance: SubTraceInvariant (TraceTypes.combine ProofEntryT.internal))
+
+noncomputable
+instance : TraceInvariant where
+  tc_inv := by dsimp only [ProofTrace.Entry, TraceTypes.ProofT]; infer_instance
+
+instance: TraceInvariant.Has ProofEntryT := inferInstanceAs (TraceInvariant.Has ProofTrace.Entry)
+
+instance: TraceInvariant.HasStep Network.ProofEntryT ProofEntryT := inferInstanceAs (TraceInvariant.HasStep (ProofEntryT.internal 0) (TraceTypes.combine ProofEntryT.internal))
+instance: TraceInvariant.HasStep Random.ProofEntryT ProofEntryT := inferInstanceAs (TraceInvariant.HasStep (ProofEntryT.internal 1) (TraceTypes.combine ProofEntryT.internal))
+instance: TraceInvariant.HasStep (ProtocolEvent.ProofEntryT Test.SignedDHEvent) ProofEntryT := inferInstanceAs (TraceInvariant.HasStep (ProofEntryT.internal 2) (TraceTypes.combine ProofEntryT.internal))
+instance: TraceInvariant.HasStep (PersistentLocalState.CompromisableState.ProofEntryT Test.ClientInitiateState) ProofEntryT := inferInstanceAs (TraceInvariant.HasStep (ProofEntryT.internal 3) (TraceTypes.combine ProofEntryT.internal))
+instance: TraceInvariant.HasStep (PersistentLocalState.CompromisableState.ProofEntryT Test.ClientFinishState) ProofEntryT := inferInstanceAs (TraceInvariant.HasStep (ProofEntryT.internal 4) (TraceTypes.combine ProofEntryT.internal))
+instance: TraceInvariant.HasStep (PersistentLocalState.CompromisableState.ProofEntryT Test.ServerFinishState) ProofEntryT := inferInstanceAs (TraceInvariant.HasStep (ProofEntryT.internal 5) (TraceTypes.combine ProofEntryT.internal))
+instance: TraceInvariant.HasStep (LongTermKeys.ProofEntryT "SignedDH") ProofEntryT := inferInstanceAs (TraceInvariant.HasStep (ProofEntryT.internal 6) (TraceTypes.combine ProofEntryT.internal))
+
+example: TraceInvariant.Has Network.ProofEntryT := inferInstance
+example: TraceInvariant.Has Random.ProofEntryT := inferInstance
+example: TraceInvariant.Has (ProtocolEvent.ProofEntryT Test.SignedDHEvent) := inferInstance
+example: TraceInvariant.Has (PersistentLocalState.CompromisableState.ProofEntryT Test.ClientInitiateState) := inferInstance
+example: TraceInvariant.Has (PersistentLocalState.CompromisableState.ProofEntryT Test.ClientFinishState) := inferInstance
+example: TraceInvariant.Has (PersistentLocalState.CompromisableState.ProofEntryT Test.ServerFinishState) := inferInstance
+example: TraceInvariant.Has (LongTermKeys.ProofEntryT "SignedDH") := inferInstance
+
+instance : ∀ id, SubBaseAttackerKnowledgeTheorem (ProofEntryT.internal id) (baseAttackerKnowledge.internal id)
+  -- TODO: investigate why infer_instance doesn't work
+  | 0 => by dsimp only [ProofEntryT.internal, baseAttackerKnowledge.internal]; apply Network.baseAttackerKnowledgeTheorem
+  | 1 => by dsimp only [ProofEntryT.internal, baseAttackerKnowledge.internal]; apply Random.baseAttackerKnowledgeTheorem
+  | 2 => by dsimp only [ProofEntryT.internal, baseAttackerKnowledge.internal]; apply ProtocolEvent.baseAttackerKnowledgeTheorem
+  | 3 => by dsimp only [ProofEntryT.internal, baseAttackerKnowledge.internal]; apply PersistentLocalState.CompromisableState.baseAttackerKnowledgeTheorem
+  | 4 => by dsimp only [ProofEntryT.internal, baseAttackerKnowledge.internal]; apply PersistentLocalState.CompromisableState.baseAttackerKnowledgeTheorem
+  | 5 => by dsimp only [ProofEntryT.internal, baseAttackerKnowledge.internal]; apply PersistentLocalState.CompromisableState.baseAttackerKnowledgeTheorem
+  | 6 => by dsimp only [ProofEntryT.internal, baseAttackerKnowledge.internal]; apply LongTermKeys.baseAttackerKnowledgeTheorem "SignedDH"
+
+instance: SubBaseAttackerKnowledgeTheorem (ProofEntryT) (baseAttackerKnowledge) := by
+  dsimp only [ProofEntryT, baseAttackerKnowledge]
+  infer_instance
+
+instance: BaseAttackerKnowledgeTheorem where
+  pf := by
+    dsimp only [ProofTrace.Entry, TraceTypes.ProofT, BaseAttackerKnowledge.attackerKnows]
+    -- TODO infer_instance
+    exact instSubBaseAttackerKnowledgeTheoremExecEntryTProofEntryTBaseAttackerKnowledge
+
+instance: (id: Fin 4) → SubAttackerKnowledgeTheorem (attackerKnowledge.internal id)
   | 0 => inferInstanceAs (SubAttackerKnowledgeTheorem Hash.attackerKnowledge)
   | 1 => inferInstanceAs (SubAttackerKnowledgeTheorem Signature.attackerKnowledge)
   | 2 => inferInstanceAs (SubAttackerKnowledgeTheorem DiffieHellman.attackerKnowledge)
+  | 3 => inferInstanceAs (SubAttackerKnowledgeTheorem Random.attackerKnowledge)
 
 instance: SubAttackerKnowledgeTheorem attackerKnowledge := inferInstanceAs (SubAttackerKnowledgeTheorem (SubAttackerKnowledge.combine attackerKnowledge.internal))
 
@@ -977,20 +1133,8 @@ instance: AttackerKnowledgeTheorem where
   inst := inferInstanceAs (SubAttackerKnowledgeTheorem attackerKnowledge)
 
 theorem test (b: Bytes) (tr: ProofTrace) :
-    tr.invariant →
-    Bytes.AttackerKnows b tr →
+    tr.Invariant →
+    Bytes.AttackerKnows b tr.erase →
     b.Publishable tr
   := by
     apply Bytes.AttackerKnows_implies_Publishable
-
-/--
-info: 'test' depends on axioms: [propext,
- Classical.choice,
- Quot.sound,
- Test.comparseExists,
- Test.event_logged_at,
- Bytes.MessageSent_implies_Publishable,
- Trace.invariant]
--/
-#guard_msgs in
-#print axioms test
