DY/Trace/Basic.lean
@@ -1,140 +1,257 @@
 module
 
-public import DY.Bytes.Basic
+meta import DY.Trace.Grind
 
 namespace DY
 
-variable [BytesFunctor]
+-- Generic trace definition
 
 public
-inductive Trace.Entry (a:Type) where
-  | rand_gen: a -> Trace.Entry a
-  | send_msg: Bytes -> Trace.Entry a
-  | log_event: Trace.Entry a
-  -- TODO
+inductive Trace (α: Type) where
+  | nil: Trace α
+  | snoc: Trace α -> α -> Trace α
 
 public
-inductive Trace (a:Type) where
-  | nil: Trace a
-  | snoc: Trace a -> Trace.Entry a -> Trace a
-
-
-namespace Trace
-
-def Entry.map
-  (f: a -> b) (e: Entry a)
-  : Entry b
-  :=
-  match e with
-  | .rand_gen pf => .rand_gen (f pf)
-  | .send_msg msg => .send_msg msg
-  | .log_event => .log_event
-
-def Trace.map
-  (f: a -> b) (tr: Trace a)
-  : Trace b
-  :=
-  match tr with
-  | .nil => .nil
-  | .snoc tr_before e => .snoc (Trace.map f tr_before) (Entry.map f e)
-
-instance : Functor Trace where
-  map := Trace.map
-
-instance : LawfulFunctor Trace where
-  map_const := by
-    intros
-    simp [Functor.mapConst, Functor.map]
-  id_map := by
-    intros α tr
-    simp [Functor.map]
-    induction tr with
-    | nil =>
-      simp [Trace.map]
-    | snoc tr_before e =>
-      simp [Trace.map, Entry.map]
-      grind
-  comp_map := by
-    intros α β γ g h tr
-    simp [Functor.map]
-    induction tr with
-    | nil =>
-      simp [Trace.map]
-    | snoc tr_before e =>
-      simp [Trace.map, Entry.map]
-      grind
+inductive Trace.le {α: Type} : Trace α -> Trace α -> Prop where
+  | equal: (tr: Trace α) -> Trace.le tr tr
+  | extend: (tr1: Trace α) -> (tr2: Trace α) -> (e: α) -> Trace.le tr1 tr2 -> Trace.le tr1 (.snoc tr2 e)
 
 public
-inductive LETrace : Trace a -> Trace a -> Prop where
-  | equal: (tr: Trace a) -> LETrace tr tr
-  | extend: (tr1: Trace a) -> (tr2: Trace a) -> (e: Entry a) -> LETrace tr1 tr2 -> LETrace tr1 (.snoc tr2 e)
+instance {α: Type}: LE (Trace α) where
+  le := Trace.le
 
+@[refl]
 public
-instance : LE (Trace a) where
-  le := LETrace
-
--- TODO: is there a typeclass about this?
-@[grind, refl]
-public
-theorem trace_le_refl
+theorem Trace.le_refl
+  {α: Type}
   (tr: Trace α)
   : tr ≤ tr
-  := by
-    exact LETrace.equal tr
+:=
+  Trace.le.equal tr
+
+grind_pattern Trace.le_refl => tr ≤ tr
 
 public
-theorem trace_le_trans
-  (tr1: Trace a) (tr2: Trace a) (tr3: Trace a)
+theorem Trace.le_trans
+  {α: Type}
+  (tr1 tr2 tr3: Trace α)
   : tr1 ≤ tr2 → tr2 ≤ tr3 → tr1 ≤ tr3
-  := by
-    intros hxy hyz
-    induction hyz with
-    | equal => simp_all
-    | extend tr3 e _ ih =>
-      exact (LETrace.extend tr1 tr3 e ih)
-
--- grind_pattern trace_le_trans => tr1 ≤ tr2, tr1 ≤ tr3
+:= by
+  intros hxy hyz
+  induction hyz with
+  | equal => exact hxy
+  | extend tr3 e _ ih =>
+    exact (Trace.le.extend tr1 tr3 e ih)
 
 public
-instance : Trans (· ≤ · : Trace a → Trace a → Prop) (· ≤ ·) (· ≤ ·) where
-  trans := by
-    intros x y z
-    exact trace_le_trans x y z
-  /-by
-    intros x y z hxy hyz
-    induction hyz with
-    | equal => simp_all
-    | extend e _ ih =>
-      exact (LETrace.extend e ih)
-      -/
-
-theorem trace_le_map
-  (f: α → β)
-  (tr1 tr2: Trace α):
-  tr1 ≤ tr2 →
-  (f <$> tr1) ≤ (f <$> tr2)
-  := by
-    intro h_le
-    induction h_le
-    · apply LETrace.equal
-    · apply LETrace.extend
-      assumption
+class IntoTraceEntry (EntryT: Type) (α: Type) where
+  make: EntryT → α
 
 public
-def erase (tr: Trace α): Trace Unit :=
-  Functor.mapConst () tr
+def Trace.append
+  {EntryT α: Type} [IntoTraceEntry EntryT α]
+  (tr: Trace α) (entry: EntryT)
+  : Trace α
+:=
+  .snoc tr (IntoTraceEntry.make entry)
 
 public
-theorem erase_idempotent (tr: Trace Unit): tr.erase = tr := by
-  unfold erase
-  simp only [LawfulFunctor.map_const]
-  apply LawfulFunctor.id_map
+def Trace.append_le
+  {EntryT α: Type} [IntoTraceEntry EntryT α]
+  (tr: Trace α) (entry: EntryT)
+  : tr ≤ tr.append entry
+:= by
+  apply Trace.le.extend
+  apply Trace.le.equal
 
 public
-theorem erase_le (tr1 tr2: Trace α)
+def Trace.length {α: Type} (tr: Trace α) : Nat :=
+  match tr with
+  | .nil => 0
+  | .snoc trBefore _ => trBefore.length + 1
+
+public
+theorem Trace.length_le
+  {α: Type} (tr1 tr2: Trace α)
   : tr1 ≤ tr2 →
-  tr1.erase ≤ tr2.erase
-  := by apply trace_le_map
+    tr1.length ≤ tr2.length
+:= by
+  intro h
+  induction h <;>
+  grind [Trace.length]
 
+grind_pattern Trace.length_le => tr1 ≤ tr2, tr1.length
 
-end DY.Trace
+public
+def Trace.prefix {α: Type} (tr: Trace α) (i: Nat): Trace α :=
+  if i = tr.length then
+    tr
+  else
+    match tr with
+    | .nil => .nil
+    | .snoc trBefore _ => trBefore.prefix i
+
+public
+theorem Trace.prefix_le
+  {α: Type}
+  (tr: Trace α) (i: Nat)
+  : tr.prefix i ≤ tr
+:= by
+  fun_induction Trace.prefix
+  · apply Trace.le_refl
+  · apply Trace.le_refl
+  · apply Trace.le.extend
+    assumption
+
+grind_pattern Trace.prefix_le => tr.prefix i
+
+@[simp, grind =]
+public
+theorem Trace.prefix_eq
+  {α: Type}
+  (tr: Trace α)
+  : tr.prefix tr.length = tr
+:= by
+  unfold Trace.prefix
+  simp
+
+public
+def Trace.at {α: Type} (tr: Trace α) (i: Nat) (h_i: i < tr.length): α :=
+  match tr with
+  | .nil => False.elim (by simp_all [Trace.length])
+  | .snoc trBefore entry =>
+    if h: i = trBefore.length then
+      entry
+    else
+      trBefore.at i (by grind [Trace.length])
+
+public
+theorem Trace.at_le
+  {α: Type} (tr1 tr2: Trace α) (i: Nat) (h_i: i < tr1.length)
+  (h_le: tr1 ≤ tr2)
+  : tr1.at i h_i = tr2.at i (by grind)
+:= by
+  induction h_le <;>
+  grind [Trace.at]
+
+grind_pattern Trace.at_le => tr1 ≤ tr2, tr1.at i h_i
+grind_pattern [grind_later] Trace.at_le => tr1 ≤ tr2, tr1.at i h_i
+
+@[expose]
+public
+def Trace.at_is
+  {EntryT α: Type} [IntoTraceEntry EntryT α]
+  (tr: Trace α) (i: Nat) (entry: EntryT)
+  : Prop
+:=
+  exists h: i < tr.length,
+  tr.at i h = IntoTraceEntry.make entry
+
+public
+theorem Trace.at_is_le
+  {EntryT α: Type} [IntoTraceEntry EntryT α]
+  (tr1 tr2: Trace α) (i: Nat) (entry: EntryT)
+  : tr1 ≤ tr2 →
+    tr1.at_is i entry →
+    tr2.at_is i entry
+:= by
+  simp only [Trace.at_is]
+  grind
+
+grind_pattern Trace.at_is_le => tr1 ≤ tr2, tr1.at_is i entry
+grind_pattern [grind_later] Trace.at_is_le => tr1 ≤ tr2, tr1.at_is i entry
+
+public
+theorem Trace.at_is_append
+  {EntryT α: Type} [IntoTraceEntry EntryT α]
+  (tr: Trace α) (entry: EntryT)
+  : (tr.append entry).at_is tr.length entry
+:= by
+  grind [Trace.append, Trace.at_is, Trace.at, Trace.length]
+
+-- Execution trace
+
+public
+class ExecTraceTypes where
+  ExecT: Type
+
+@[expose]
+public
+def ExecTrace.Entry [ExecTraceTypes] := ExecTraceTypes.ExecT
+
+public
+abbrev ExecTrace [ExecTraceTypes] := Trace ExecTrace.Entry
+
+public
+class ExecTraceTypes.Has [ExecTraceTypes] (ExecEntryT: Type) where
+  inj: ExecEntryT → ExecTrace.Entry
+  proj: ExecTrace.Entry → Option ExecEntryT
+  inj_proj_eq: ∀ x y, (proj x = some y) = (x = inj y)
+
+public
+class ExecTraceTypes.HasStep (ExecEntryT1: Type) (ExecEntryT2: semiOutParam Type) where
+  inj: ExecEntryT1 → ExecEntryT2
+  proj: ExecEntryT2 → Option ExecEntryT1
+  inj_proj_eq: ∀ x y, (proj x = some y) = (x = inj y)
+
+public
+instance instExecTraceTypesHasItself [ExecTraceTypes]: ExecTraceTypes.Has ExecTrace.Entry where
+  inj x := x
+  proj x := some x
+  inj_proj_eq := by grind
+
+public
+instance instExecTraceTypesHasStep
+  [ExecTraceTypes]
+  (ExecEntryT1 ExecEntryT2: Type)
+  [ExecTraceTypes.HasStep ExecEntryT1 ExecEntryT2]
+  [ExecTraceTypes.Has ExecEntryT2]
+  : ExecTraceTypes.Has ExecEntryT1
+where
+  inj x := ExecTraceTypes.Has.inj (ExecTraceTypes.HasStep.inj (ExecEntryT2 := ExecEntryT2) x)
+  proj x :=
+    match ExecTraceTypes.Has.proj (ExecEntryT := ExecEntryT2) x with
+    | none => none
+    | some y => ExecTraceTypes.HasStep.proj y
+  inj_proj_eq x y := by
+    have := ExecTraceTypes.Has.inj_proj_eq (ExecEntryT := ExecEntryT2) x
+    have := ExecTraceTypes.HasStep.inj_proj_eq (ExecEntryT1 := ExecEntryT1) (ExecEntryT2 := ExecEntryT2)
+    grind
+
+public
+instance [ExecTraceTypes] (ExecEntryT: Type) [ExecTraceTypes.Has ExecEntryT]: IntoTraceEntry ExecEntryT ExecTrace.Entry where
+  make entry := ExecTraceTypes.Has.inj entry
+
+@[grind inj]
+public
+theorem ExecTraceTypes.Has.inj_injective
+  [ExecTraceTypes] (ExecEntryT: Type) [ExecTraceTypes.Has ExecEntryT]
+  : Function.Injective (ExecTraceTypes.Has.inj (ExecEntryT := ExecEntryT))
+:= by
+  intro x1 x2
+  have := ExecTraceTypes.Has.inj_proj_eq (ExecTraceTypes.Has.inj x1) x1
+  have := ExecTraceTypes.Has.inj_proj_eq (ExecTraceTypes.Has.inj x2) x2
+  grind
+
+public
+structure ExecTraceTypes.combine {n: Nat} (ExecTypes: Fin n → Type): Type where
+  id: Fin n
+  entry: ExecTypes id
+
+public
+instance instExecTraceTypesCombineHasStep
+  {n: Nat}
+  (Types: Fin n → Type)
+  (id: Fin n)
+  : ExecTraceTypes.HasStep (Types id) (ExecTraceTypes.combine Types) where
+  inj entry := { id, entry }
+  proj entry :=
+    if h: entry.id = id then
+      some (h ▸ entry.entry)
+    else
+      none
+  inj_proj_eq x y := by
+    cases x
+    grind
+
+end DY
