DY/Actions/Network.lean
@@ -1,0 +1,102 @@
+module
+
+public import DY.Trace
+public import DY.Bytes
+import DY.Step.Init
+
+namespace DY.Network
+
+variable [BytesFunctor]
+
+section Execution
+
+public
+structure ExecEntryT where
+  msg: Bytes
+
+public
+def baseAttackerKnowledge [ExecTraceTypes]: SubBaseAttackerKnowledge ExecEntryT where
+  attackerKnows _ entry msg := msg = entry.msg
+
+public
+def sendMessage [BytesFunctor] [ExecTraceTypes] [ExecTraceTypes.Has ExecEntryT] (msg: Bytes): Traceful Nat :=
+  do
+  let entry: ExecEntryT := ExecEntryT.mk msg
+  appendEntry entry
+
+public
+def receiveMessage [BytesFunctor] [ExecTraceTypes] [ExecTraceTypes.Has ExecEntryT] (timestamp: Nat): Traceful Bytes :=
+  do
+  let msg: ExecEntryT ← getEntry timestamp
+  return msg.msg
+
+end Execution
+
+section Proof
+
+public
+abbrev ProofEntryT := ExecEntryT
+
+public
+instance: ErasableProofEntry ExecEntryT ProofEntryT := ErasableProofEntry.default ExecEntryT
+
+public
+instance
+  [TraceTypes] [BytesInvariants]
+  : SubTraceInvariant ProofEntryT
+where
+  invariant tr entry :=
+    entry.msg.Publishable tr
+
+public
+instance baseAttackerKnowledgeTheorem
+  [TraceInvariant] [BytesInvariants]
+  [TraceTypes.Has ProofEntryT]
+  [TraceInvariant.Has ProofEntryT]:
+  SubBaseAttackerKnowledgeTheorem ProofEntryT baseAttackerKnowledge
+where
+  pf trBefore entry b := by
+    simp [SubTraceInvariant.invariant, baseAttackerKnowledge, ErasableProofEntry.erase]
+    grind
+
+@[instance]
+public
+theorem sendMessage.spec
+  [TraceInvariant]
+  [BytesInvariants] [BytesInvariantsProofs]
+  [TraceTypes.Has ProofEntryT] [TraceInvariant.Has ProofEntryT]
+  (msg: Bytes)
+  : HoareTriple
+    (sendMessage msg)
+    (fun tr => msg.Publishable tr)
+    (fun _ _ => True)
+:= by
+  apply HoareTriple.mk
+  unfold sendMessage
+  dsimp only
+  step with ⟨ fun _ => ExecEntryT.mk msg ⟩ by simp_all [ErasableProofEntry.erase, SubTraceInvariant.invariant]
+  trivial
+
+@[instance]
+public
+theorem receiveMessage.spec
+  [TraceInvariant]
+  [BytesInvariants] [BytesInvariantsProofs]
+  [TraceTypes.Has ProofEntryT] [TraceInvariant.Has ProofEntryT]
+  (timestamp: Nat)
+  : HoareTriple
+    (receiveMessage timestamp)
+    (fun _ => True)
+    (fun msg tr => msg.Publishable tr)
+:= by
+  apply HoareTriple.mk
+  unfold receiveMessage
+  step
+  have: msg.msg.Publishable tr := by simp_all [ErasableProofEntry.erase, SubTraceInvariant.invariant]; grind
+  rename_i h_msg; clear h_msg
+  step
+  grind
+
+end Proof
+
+end DY.Network
