DY/Actions/PersistentGlobalState.lean
@@ -1,0 +1,480 @@
+module
+
+public import DY.Trace
+public import DY.Bytes
+public import DY.Actions.Network -- for compromise
+public import DY.Actions.ProtocolEvent -- for compromise
+public import DY.Comparse -- for compromise
+import DY.Step.Init
+
+namespace DY.PersistentGlobalState
+
+section State
+
+section Execution
+
+namespace State
+
+public
+structure ExecEntryT (StateT: Type) where
+  st: StateT
+
+public
+def baseAttackerKnowledge [BytesFunctor] [ExecTraceTypes] (StateT: Type): SubBaseAttackerKnowledge (ExecEntryT StateT) where
+  attackerKnows _ _ _ := False
+
+end State
+
+public
+def storeGlobalState
+  {StateT: Type}
+  [ExecTraceTypes] [ExecTraceTypes.Has (State.ExecEntryT StateT)]
+  (st: StateT)
+  : Traceful Nat
+:= do
+  let entry: State.ExecEntryT StateT := { st }
+  appendEntry entry
+
+public
+def getGlobalState
+  {StateT: Type}
+  [ExecTraceTypes] [ExecTraceTypes.Has (State.ExecEntryT StateT)]
+  (i: Nat)
+  : Traceful StateT
+:= do
+  let e: State.ExecEntryT StateT ← getEntry i
+  return e.st
+
+end Execution
+
+section Proof
+
+public
+class GlobalStateInv [TraceTypes] (StateT: Type) where
+  invariant: StateT → ProofTrace → Prop
+  invariant_later: ∀ st tr1 tr2,
+    tr1 ≤ tr2 →
+    invariant st tr1 →
+    invariant st tr2
+
+grind_pattern GlobalStateInv.invariant_later => tr1 ≤ tr2, GlobalStateInv.invariant st tr1
+grind_pattern [grind_later] GlobalStateInv.invariant_later => tr1 ≤ tr2, GlobalStateInv.invariant st tr1
+
+namespace State
+
+public
+abbrev ProofEntryT (StateT: Type) := ExecEntryT StateT
+
+public
+instance (StateT: Type): ErasableProofEntry (ExecEntryT StateT) (ProofEntryT StateT) := ErasableProofEntry.default (ExecEntryT StateT)
+
+public
+instance
+  [TraceTypes]
+  (StateT: Type)
+  [GlobalStateInv StateT]
+  : SubTraceInvariant (ProofEntryT StateT)
+where
+  invariant tr entry :=
+    GlobalStateInv.invariant entry.st tr
+
+public
+instance baseAttackerKnowledgeTheorem
+  [TraceInvariant] [BytesFunctor] [BytesInvariants]
+  (StateT: Type)
+  [TraceTypes.Has (ProofEntryT StateT)]
+  [GlobalStateInv StateT]
+  [TraceInvariant.Has (ProofEntryT StateT)]
+  : SubBaseAttackerKnowledgeTheorem (ProofEntryT StateT) (baseAttackerKnowledge StateT)
+where
+  pf trBefore entry b := by
+    simp [baseAttackerKnowledge]
+
+end State
+
+@[instance]
+public
+theorem storeGlobalState.spec
+  {StateT: Type}
+  [TraceInvariant]
+  [GlobalStateInv StateT]
+  [TraceTypes.Has (State.ProofEntryT StateT)] [TraceInvariant.Has (State.ProofEntryT StateT)]
+  (st: StateT)
+  : HoareTriple
+    (storeGlobalState st)
+    (fun tr => GlobalStateInv.invariant st tr)
+    (fun _ _ => True)
+:= by
+  apply HoareTriple.mk
+  unfold storeGlobalState
+  dsimp only
+  step with ⟨ fun _ => State.ExecEntryT.mk st ⟩ by simp_all [ErasableProofEntry.erase, SubTraceInvariant.invariant]
+  trivial
+
+@[instance]
+public
+theorem getGlobalState.spec
+  {StateT: Type}
+  [TraceInvariant]
+  [GlobalStateInv StateT]
+  [TraceTypes.Has (State.ProofEntryT StateT)] [TraceInvariant.Has (State.ProofEntryT StateT)]
+  (i: Nat)
+  : HoareTriple
+    (getGlobalState i: Traceful StateT)
+    (fun _ => True)
+    (fun st tr => GlobalStateInv.invariant st tr)
+:= by
+  apply HoareTriple.mk
+  unfold getGlobalState
+  step
+  have: GlobalStateInv.invariant e.st tr := by simp_all [ErasableProofEntry.erase, SubTraceInvariant.invariant]; grind
+  rename_i h; clear h
+  step
+  grind
+
+end Proof
+
+end State
+
+section Compromise
+
+section Execution
+
+namespace Compromise
+
+public
+structure CompromiseEvent (StateT: Type) where
+  state: StateT
+
+@[expose]
+public
+def ExecEntryT.internal (StateT: Type): Fin 1 → Type
+  | 0 => ProtocolEvent.ExecEntryT (CompromiseEvent StateT)
+
+@[expose, implicit_reducible]
+public
+def ExecEntryT (StateT: Type): Type :=
+  ExecTraceTypes.combine (ExecEntryT.internal StateT)
+
+public
+instance (StateT: Type): ExecTraceTypes.HasStep (ProtocolEvent.ExecEntryT (CompromiseEvent StateT)) (ExecEntryT StateT) :=
+  inferInstanceAs (ExecTraceTypes.HasStep (ExecEntryT.internal StateT 0) (ExecTraceTypes.combine (ExecEntryT.internal StateT)))
+
+public
+def baseAttackerKnowledge.internal [BytesFunctor] [ExecTraceTypes] (StateT: Type): (id: Fin 1) → SubBaseAttackerKnowledge (ExecEntryT.internal StateT id)
+  | 0 => ProtocolEvent.baseAttackerKnowledge (CompromiseEvent StateT)
+
+public
+def baseAttackerKnowledge [BytesFunctor] [ExecTraceTypes] (StateT: Type): SubBaseAttackerKnowledge (ExecEntryT StateT) :=
+  SubBaseAttackerKnowledge.combine (baseAttackerKnowledge.internal StateT)
+
+end Compromise
+
+public
+def compromise
+  (StateT: Type)
+  [BytesFunctor]
+  [Comparse.ParseableSerializeable StateT]
+  [ExecTraceTypes]
+  [ExecTraceTypes.Has Network.ExecEntryT]
+  [ExecTraceTypes.Has (State.ExecEntryT StateT)]
+  [ExecTraceTypes.Has (Compromise.ExecEntryT StateT)]
+  (i: Nat)
+  : Traceful Nat
+:= do
+  let state: StateT ← getGlobalState i
+  ProtocolEvent.logEvent ({ state }: Compromise.CompromiseEvent StateT)
+  Network.sendMessage (Comparse.ParseableSerializeable.serialize state)
+
+public
+def GlobalStateCompromised
+  {StateT: Type}
+  [ExecTraceTypes] [ExecTraceTypes.Has (Compromise.ExecEntryT StateT)]
+  (state: StateT)
+  (tr: ExecTrace)
+  : Prop
+:=
+  tr.EventLogged ({ state }: Compromise.CompromiseEvent StateT)
+
+public
+theorem GlobalStateCompromised_le
+  {StateT: Type}
+  [ExecTraceTypes] [ExecTraceTypes.Has (Compromise.ExecEntryT StateT)]
+  (state: StateT)
+  (tr1 tr2: ExecTrace)
+  : tr1 ≤ tr2 →
+    GlobalStateCompromised state tr1 →
+    GlobalStateCompromised state tr2
+:= by
+  simp [GlobalStateCompromised]
+  grind
+
+grind_pattern GlobalStateCompromised_le => tr1 ≤ tr2, GlobalStateCompromised state tr1
+grind_pattern [grind_later] GlobalStateCompromised_le => tr1 ≤ tr2, GlobalStateCompromised state tr1
+
+end Execution
+
+section Proof
+
+namespace Compromise
+
+@[expose]
+public
+def ProofEntryT.internal (StateT: Type): Fin 1 → Type
+  | 0 => ProtocolEvent.ProofEntryT (Compromise.CompromiseEvent StateT)
+
+@[expose, implicit_reducible]
+public
+def ProofEntryT (StateT: Type): Type :=
+  TraceTypes.combine (ProofEntryT.internal StateT)
+
+public
+instance (StateT: Type): ∀ id, ErasableProofEntry (ExecEntryT.internal StateT id) (ProofEntryT.internal StateT id)
+  | 0 => by dsimp only [ExecEntryT.internal, ProofEntryT.internal]; infer_instance
+
+public
+instance (StateT: Type): ErasableProofEntry (ExecEntryT StateT) (ProofEntryT StateT) :=
+  (inferInstance: ErasableProofEntry (ExecTraceTypes.combine (ExecEntryT.internal StateT)) (TraceTypes.combine (ProofEntryT.internal StateT)))
+
+public
+instance (StateT: Type): TraceTypes.HasStep (ProtocolEvent.ProofEntryT (CompromiseEvent StateT)) (ProofEntryT StateT) :=
+  inferInstanceAs (TraceTypes.HasStep (ProofEntryT.internal StateT 0) (TraceTypes.combine (ProofEntryT.internal StateT)))
+
+public
+instance
+  {StateT: Type}
+  [TraceTypes]
+  : ProtocolEvent.EventInv (CompromiseEvent StateT)
+where
+  invariant _ _ := True
+
+public
+instance [TraceTypes] (StateT: Type): ∀ id, SubTraceInvariant (ProofEntryT.internal StateT id)
+  | 0 => by dsimp only [ProofEntryT.internal]; infer_instance
+
+public
+instance [TraceTypes] (StateT: Type): SubTraceInvariant (ProofEntryT StateT) :=
+  (inferInstance: SubTraceInvariant (TraceTypes.combine (ProofEntryT.internal StateT)))
+
+public
+instance [TraceTypes] (StateT: Type): TraceInvariant.HasStep (ProtocolEvent.ProofEntryT (CompromiseEvent StateT)) (ProofEntryT StateT) :=
+  inferInstanceAs (TraceInvariant.HasStep (ProofEntryT.internal StateT 0) (TraceTypes.combine (ProofEntryT.internal StateT)))
+
+public
+instance
+  [TraceInvariant] [BytesFunctor] [BytesInvariants]
+  (StateT: Type)
+  [TraceTypes.Has (ProofEntryT StateT)]
+  [TraceInvariant.Has (ProofEntryT StateT)]
+  : ∀ id, SubBaseAttackerKnowledgeTheorem (ProofEntryT.internal StateT id) (baseAttackerKnowledge.internal StateT id)
+  -- TODO: investigate why infer_instance doesn't work
+  | 0 => by dsimp only [ProofEntryT.internal, baseAttackerKnowledge.internal]; apply ProtocolEvent.baseAttackerKnowledgeTheorem
+
+public
+instance baseAttackerKnowledgeTheorem
+  [TraceInvariant] [BytesFunctor] [BytesInvariants]
+  (StateT: Type)
+  [TraceTypes.Has (ProofEntryT StateT)]
+  [TraceInvariant.Has (ProofEntryT StateT)]
+  : SubBaseAttackerKnowledgeTheorem (ProofEntryT StateT) (baseAttackerKnowledge StateT)
+:= by
+  dsimp only [ProofEntryT, baseAttackerKnowledge]
+  apply instSubBaseAttackerKnowledgeTheoremCombine
+
+end Compromise
+
+public
+def label
+  {StateT: Type}
+  [ExecTraceTypes] [ExecTraceTypes.Has (Compromise.ExecEntryT StateT)]
+  (state: StateT)
+:=
+  ProtocolEvent.label ({ state }: Compromise.CompromiseEvent StateT)
+
+public
+theorem label_isCorrupt
+  {StateT: Type}
+  [ExecTraceTypes] [ExecTraceTypes.Has (Compromise.ExecEntryT StateT)]
+  (state: StateT)
+  (tr: ExecTrace)
+  : (label state).isCorrupt tr = GlobalStateCompromised state tr
+:= by
+  grind [label, GlobalStateCompromised]
+
+grind_pattern label_isCorrupt => (label state).isCorrupt tr
+
+public
+class CompromisableGlobalStateInv
+  (StateT: Type)
+  [TraceTypes]
+  [BytesFunctor] [BytesInvariants]
+  [Comparse.ParseableSerializeable StateT]
+  [ExecTraceTypes.Has (Compromise.ExecEntryT StateT)]
+extends
+  GlobalStateInv StateT
+where
+  invariant_implies_KnowableBy:
+    ∀ (state: StateT) tr,
+      GlobalStateInv.invariant state tr →
+      Comparse.isWellFormed (Bytes.KnowableBy (label state)) state tr
+
+@[instance]
+public
+theorem compromise.spec
+  {StateT: Type}
+  [BytesFunctor]
+  [Comparse.ParseableSerializeable StateT]
+  [TraceInvariant]
+  [TraceTypes.Has Network.ProofEntryT]
+  [TraceTypes.Has (State.ProofEntryT StateT)]
+  [TraceTypes.Has (Compromise.ProofEntryT StateT)]
+  [BytesInvariants] [BytesInvariantsProofs]
+  [Comparse.ParseableSerializeable StateT]
+  [CompromisableGlobalStateInv StateT]
+  [TraceInvariant.Has Network.ProofEntryT]
+  [TraceInvariant.Has (State.ProofEntryT StateT)]
+  [TraceInvariant.Has (Compromise.ProofEntryT StateT)]
+  (i: Nat)
+  : HoareTriple
+    (compromise StateT i)
+    (fun _ => True)
+    (fun _ _ => True)
+:= by
+  apply HoareTriple.mk
+  unfold compromise
+  step
+  step by simp [ProtocolEvent.EventInv.invariant]
+  step by
+    have := CompromisableGlobalStateInv.invariant_implies_KnowableBy state tr
+    have : (label state).isCorrupt tr.erase := by simp_all [label, ProtocolEvent.label_isCorrupt]
+    grind [Comparse.isWellFormed, canFlowTrans]
+  trivial
+
+end Proof
+
+end Compromise
+
+section CompromisableState
+
+namespace CompromisableState
+
+@[expose]
+public
+def ExecEntryT.internal (StateT: Type): Fin 2 → Type
+  | 0 => State.ExecEntryT StateT
+  | 1 => Compromise.ExecEntryT StateT
+
+@[expose, implicit_reducible]
+public
+def ExecEntryT (StateT: Type): Type :=
+  ExecTraceTypes.combine (ExecEntryT.internal StateT)
+
+public
+instance (StateT: Type): ExecTraceTypes.HasStep (State.ExecEntryT StateT) (ExecEntryT StateT) :=
+  inferInstanceAs (ExecTraceTypes.HasStep (ExecEntryT.internal StateT 0) (ExecTraceTypes.combine (ExecEntryT.internal StateT)))
+
+public
+instance (StateT: Type): ExecTraceTypes.HasStep (Compromise.ExecEntryT StateT) (ExecEntryT StateT) :=
+  inferInstanceAs (ExecTraceTypes.HasStep (ExecEntryT.internal StateT 1) (ExecTraceTypes.combine (ExecEntryT.internal StateT)))
+
+public
+def baseAttackerKnowledge.internal [BytesFunctor] [ExecTraceTypes] (StateT: Type): (id: Fin 2) → SubBaseAttackerKnowledge (ExecEntryT.internal StateT id)
+  | 0 => State.baseAttackerKnowledge StateT
+  | 1 => Compromise.baseAttackerKnowledge StateT
+
+public
+def baseAttackerKnowledge [BytesFunctor] [ExecTraceTypes] (StateT: Type): SubBaseAttackerKnowledge (ExecEntryT StateT) :=
+  SubBaseAttackerKnowledge.combine (baseAttackerKnowledge.internal StateT)
+
+@[expose]
+public
+def ProofEntryT.internal (StateT: Type): Fin 2 → Type
+  | 0 => State.ProofEntryT StateT
+  | 1 => Compromise.ProofEntryT StateT
+
+@[expose, implicit_reducible]
+public
+def ProofEntryT (StateT: Type): Type :=
+  TraceTypes.combine (ProofEntryT.internal StateT)
+
+public
+instance (StateT: Type): ∀ id, ErasableProofEntry (ExecEntryT.internal StateT id) (ProofEntryT.internal StateT id)
+  | 0 | 1 => by dsimp only [ExecEntryT.internal, ProofEntryT.internal]; infer_instance
+
+public
+instance (StateT: Type): ErasableProofEntry (ExecEntryT StateT) (ProofEntryT StateT) :=
+  (inferInstance: ErasableProofEntry (ExecTraceTypes.combine (ExecEntryT.internal StateT)) (TraceTypes.combine (ProofEntryT.internal StateT)))
+
+public
+instance (StateT: Type): TraceTypes.HasStep (State.ProofEntryT StateT) (ProofEntryT StateT) :=
+  inferInstanceAs (TraceTypes.HasStep (ProofEntryT.internal StateT 0) (TraceTypes.combine (ProofEntryT.internal StateT)))
+
+public
+instance (StateT: Type): TraceTypes.HasStep (Compromise.ProofEntryT StateT) (ProofEntryT StateT) :=
+  inferInstanceAs (TraceTypes.HasStep (ProofEntryT.internal StateT 1) (TraceTypes.combine (ProofEntryT.internal StateT)))
+
+public
+instance
+  [TraceTypes] [BytesFunctor] [BytesInvariants]
+  (StateT: Type) [Comparse.ParseableSerializeable StateT] [ExecTraceTypes.Has (ExecEntryT StateT)]
+  [CompromisableGlobalStateInv StateT]
+  : ∀ id, SubTraceInvariant (ProofEntryT.internal StateT id)
+  | 0 | 1 => by dsimp only [ProofEntryT.internal]; infer_instance
+
+public
+instance
+  [TraceTypes] [BytesFunctor] [BytesInvariants]
+  (StateT: Type) [Comparse.ParseableSerializeable StateT] [ExecTraceTypes.Has (ExecEntryT StateT)]
+  [CompromisableGlobalStateInv StateT]
+  : SubTraceInvariant (ProofEntryT StateT)
+:=
+  (inferInstance: SubTraceInvariant (TraceTypes.combine (ProofEntryT.internal StateT)))
+
+public
+instance
+  [TraceTypes] [BytesFunctor] [BytesInvariants]
+  (StateT: Type) [Comparse.ParseableSerializeable StateT] [ExecTraceTypes.Has (ExecEntryT StateT)]
+  [CompromisableGlobalStateInv StateT]
+  : TraceInvariant.HasStep (State.ProofEntryT StateT) (ProofEntryT StateT)
+:=
+  inferInstanceAs (TraceInvariant.HasStep (ProofEntryT.internal StateT 0) (TraceTypes.combine (ProofEntryT.internal StateT)))
+
+public
+instance
+  [TraceTypes] [BytesFunctor] [BytesInvariants]
+  (StateT: Type) [Comparse.ParseableSerializeable StateT] [ExecTraceTypes.Has (ExecEntryT StateT)]
+  [CompromisableGlobalStateInv StateT]
+  : TraceInvariant.HasStep (Compromise.ProofEntryT StateT) (ProofEntryT StateT)
+:=
+  inferInstanceAs (TraceInvariant.HasStep (ProofEntryT.internal StateT 1) (TraceTypes.combine (ProofEntryT.internal StateT)))
+
+public
+instance
+  [TraceInvariant] [BytesFunctor] [BytesInvariants]
+  (StateT: Type) [Comparse.ParseableSerializeable StateT]
+  [TraceTypes.Has (ProofEntryT StateT)]
+  [CompromisableGlobalStateInv StateT]
+  [TraceInvariant.Has (ProofEntryT StateT)]
+  : ∀ id, SubBaseAttackerKnowledgeTheorem (ProofEntryT.internal StateT id) (baseAttackerKnowledge.internal StateT id)
+  -- TODO: investigate why infer_instance doesn't work
+  | 0 => by dsimp only [ProofEntryT.internal, baseAttackerKnowledge.internal]; apply State.baseAttackerKnowledgeTheorem
+  | 1 => by dsimp only [ProofEntryT.internal, baseAttackerKnowledge.internal]; apply Compromise.baseAttackerKnowledgeTheorem
+
+public
+instance baseAttackerKnowledgeTheorem
+  [TraceInvariant] [BytesFunctor] [BytesInvariants]
+  (StateT: Type) [Comparse.ParseableSerializeable StateT]
+  [TraceTypes.Has (ProofEntryT StateT)]
+  [CompromisableGlobalStateInv StateT]
+  [TraceInvariant.Has (ProofEntryT StateT)]
+  : SubBaseAttackerKnowledgeTheorem (ProofEntryT StateT) (baseAttackerKnowledge StateT)
+:= by
+  dsimp only [ProofEntryT, baseAttackerKnowledge]
+  apply instSubBaseAttackerKnowledgeTheoremCombine -- infer_instance?
+
+
+end CompromisableState
+
+end CompromisableState
+
+end DY.PersistentGlobalState
