DY/Actions/PersistentLocalState.lean
@@ -1,0 +1,548 @@
+module
+
+public import DY.Trace
+public import DY.Bytes
+public import DY.Actions.PersistentGlobalState
+import DY.Step.Init
+
+namespace DY
+
+public
+abbrev Participant := String
+
+namespace PersistentLocalState
+
+section State
+
+section Execution
+
+public
+structure LocalState (StateT: Type) where
+  participant: Participant
+  state: StateT
+
+noncomputable
+instance
+  [BytesFunctor]
+  (StateT: Type)
+  [Comparse.ParseableSerializeable StateT]: Comparse.ParseableSerializeable (LocalState StateT) := Comparse.comparseMetaProgramExists
+
+namespace State
+
+@[expose]
+public
+def ExecEntryT.internal (StateT: Type): Fin 1 → Type
+  | 0 => PersistentGlobalState.State.ExecEntryT (LocalState StateT)
+
+@[expose, implicit_reducible]
+public
+def ExecEntryT (StateT: Type): Type :=
+  ExecTraceTypes.combine (ExecEntryT.internal StateT)
+
+public
+instance (StateT: Type): ExecTraceTypes.HasStep (PersistentGlobalState.State.ExecEntryT (LocalState StateT)) (ExecEntryT StateT) :=
+  inferInstanceAs (ExecTraceTypes.HasStep (ExecEntryT.internal StateT 0) (ExecTraceTypes.combine (ExecEntryT.internal StateT)))
+
+public
+def baseAttackerKnowledge.internal [BytesFunctor] [ExecTraceTypes] (StateT: Type): (id: Fin 1) → SubBaseAttackerKnowledge (ExecEntryT.internal StateT id)
+  | 0 => PersistentGlobalState.State.baseAttackerKnowledge (LocalState StateT)
+
+public
+def baseAttackerKnowledge [BytesFunctor] [ExecTraceTypes] (StateT: Type): SubBaseAttackerKnowledge (ExecEntryT StateT) :=
+  SubBaseAttackerKnowledge.combine (baseAttackerKnowledge.internal StateT)
+
+end State
+
+public
+def storeLocalState
+  {StateT: Type}
+  [ExecTraceTypes] [ExecTraceTypes.Has (State.ExecEntryT StateT)]
+  (participant: Participant) (state: StateT)
+  : Traceful Nat
+:= do
+  PersistentGlobalState.storeGlobalState ({ participant, state }: LocalState StateT)
+
+public
+def getLocalState
+  {StateT: Type}
+  [ExecTraceTypes] [ExecTraceTypes.Has (State.ExecEntryT StateT)]
+  (participant: Participant) (i: Nat)
+  : Traceful StateT
+:= do
+  let st: LocalState StateT ← PersistentGlobalState.getGlobalState i
+  guard (st.participant = participant)
+  return st.state
+
+end Execution
+
+section Proof
+
+public
+class LocalStateInv [TraceTypes] (StateT: Type) where
+  invariant: Participant → StateT → ProofTrace → Prop
+  invariant_later: ∀ p st tr1 tr2,
+    tr1 ≤ tr2 →
+    invariant p st tr1 →
+    invariant p st tr2
+
+grind_pattern LocalStateInv.invariant_later => tr1 ≤ tr2, LocalStateInv.invariant p st tr1
+grind_pattern [grind_later] LocalStateInv.invariant_later => tr1 ≤ tr2, LocalStateInv.invariant p st tr1
+
+namespace State
+
+@[expose]
+public
+def ProofEntryT.internal (StateT: Type): Fin 1 → Type
+  | 0 => PersistentGlobalState.State.ProofEntryT (LocalState StateT)
+
+public
+abbrev ProofEntryT (StateT: Type): Type :=
+  TraceTypes.combine (ProofEntryT.internal StateT)
+
+public
+instance (StateT: Type): ∀ id, ErasableProofEntry (ExecEntryT.internal StateT id) (ProofEntryT.internal StateT id)
+  | 0 => by dsimp only [ExecEntryT.internal, ProofEntryT.internal]; infer_instance
+
+public
+instance (StateT: Type): ErasableProofEntry (ExecEntryT StateT) (ProofEntryT StateT) :=
+  (inferInstance: ErasableProofEntry (ExecTraceTypes.combine (ExecEntryT.internal StateT)) (TraceTypes.combine (ProofEntryT.internal StateT)))
+
+public
+instance (StateT: Type): TraceTypes.HasStep (PersistentGlobalState.State.ProofEntryT (LocalState StateT)) (ProofEntryT StateT) :=
+  inferInstanceAs (TraceTypes.HasStep (ProofEntryT.internal StateT 0) (TraceTypes.combine (ProofEntryT.internal StateT)))
+
+public
+instance
+  [TraceTypes]
+  (StateT: Type) [LocalStateInv StateT]
+  : PersistentGlobalState.GlobalStateInv (LocalState StateT)
+where
+  invariant st tr := LocalStateInv.invariant st.participant st.state tr
+  invariant_later st tr1 tr2 := LocalStateInv.invariant_later st.participant st.state tr1 tr2
+
+public
+instance [TraceTypes] (StateT: Type) [LocalStateInv StateT]: ∀ id, SubTraceInvariant (ProofEntryT.internal StateT id)
+  | 0 => by dsimp only [ProofEntryT.internal]; infer_instance
+
+public
+instance [TraceTypes] (StateT: Type) [LocalStateInv StateT]: SubTraceInvariant (ProofEntryT StateT) :=
+  (inferInstance: SubTraceInvariant (TraceTypes.combine (ProofEntryT.internal StateT)))
+
+public
+instance [TraceTypes] (StateT: Type) [LocalStateInv StateT]: TraceInvariant.HasStep (PersistentGlobalState.State.ProofEntryT (LocalState StateT)) (ProofEntryT StateT) :=
+  inferInstanceAs (TraceInvariant.HasStep (ProofEntryT.internal StateT 0) (TraceTypes.combine (ProofEntryT.internal StateT)))
+
+public
+instance
+  [TraceInvariant] [BytesFunctor] [BytesInvariants]
+  (StateT: Type)
+  [LocalStateInv StateT]
+  [TraceTypes.Has (ProofEntryT StateT)]
+  [TraceInvariant.Has (ProofEntryT StateT)]
+  : ∀ id, SubBaseAttackerKnowledgeTheorem (ProofEntryT.internal StateT id) (baseAttackerKnowledge.internal StateT id)
+  -- TODO: investigate why infer_instance doesn't work
+  | 0 => by dsimp only [ProofEntryT.internal, baseAttackerKnowledge.internal]; apply PersistentGlobalState.State.baseAttackerKnowledgeTheorem
+
+public
+instance baseAttackerKnowledgeTheorem
+  [TraceInvariant] [BytesFunctor] [BytesInvariants]
+  (StateT: Type)
+  [LocalStateInv StateT]
+  [TraceTypes.Has (ProofEntryT StateT)]
+  [TraceInvariant.Has (ProofEntryT StateT)]
+  : SubBaseAttackerKnowledgeTheorem (ProofEntryT StateT) (baseAttackerKnowledge StateT)
+:= by
+  dsimp only [ProofEntryT, baseAttackerKnowledge]
+  apply instSubBaseAttackerKnowledgeTheoremCombine
+
+end State
+
+@[instance]
+public
+theorem storeLocalState.spec
+  {StateT: Type}
+  [TraceInvariant]
+  [LocalStateInv StateT]
+  [TraceTypes.Has (State.ProofEntryT StateT)] [TraceInvariant.Has (State.ProofEntryT StateT)]
+  (participant: Participant) (state: StateT)
+  : HoareTriple
+    (storeLocalState participant state)
+    (fun tr => LocalStateInv.invariant participant state tr)
+    (fun _ _ => True)
+:= by
+  apply HoareTriple.mk
+  unfold storeLocalState
+  step by simp_all [PersistentGlobalState.GlobalStateInv.invariant]
+  trivial
+
+@[instance]
+public
+theorem getLocalState.spec
+  {StateT: Type}
+  [TraceInvariant]
+  [LocalStateInv StateT]
+  [TraceTypes.Has (State.ProofEntryT StateT)] [TraceInvariant.Has (State.ProofEntryT StateT)]
+  (participant: Participant) (i: Nat)
+  : HoareTriple
+    (getLocalState participant i: Traceful StateT)
+    (fun _ => True)
+    (fun st tr => LocalStateInv.invariant participant st tr)
+:= by
+  apply HoareTriple.mk
+  unfold getLocalState
+  step
+  step
+  step
+  simp_all [PersistentGlobalState.GlobalStateInv.invariant]
+
+end Proof
+
+end State
+
+section Compromise
+
+section Execution
+
+namespace Compromise
+
+@[expose]
+public
+def ExecEntryT.internal (StateT: Type): Fin 1 → Type
+  | 0 => PersistentGlobalState.Compromise.ExecEntryT (LocalState StateT)
+
+@[expose, implicit_reducible]
+public
+def ExecEntryT (StateT: Type): Type :=
+  ExecTraceTypes.combine (ExecEntryT.internal StateT)
+
+public
+instance (StateT: Type): ExecTraceTypes.HasStep (PersistentGlobalState.Compromise.ExecEntryT (LocalState StateT)) (ExecEntryT StateT) :=
+  inferInstanceAs (ExecTraceTypes.HasStep (ExecEntryT.internal StateT 0) (ExecTraceTypes.combine (ExecEntryT.internal StateT)))
+
+public
+def baseAttackerKnowledge.internal [BytesFunctor] [ExecTraceTypes] (StateT: Type): (id: Fin 1) → SubBaseAttackerKnowledge (ExecEntryT.internal StateT id)
+  | 0 => PersistentGlobalState.Compromise.baseAttackerKnowledge (LocalState StateT)
+
+public
+def baseAttackerKnowledge [BytesFunctor] [ExecTraceTypes] (StateT: Type): SubBaseAttackerKnowledge (ExecEntryT StateT) :=
+  SubBaseAttackerKnowledge.combine (baseAttackerKnowledge.internal StateT)
+
+end Compromise
+
+public
+noncomputable
+def compromise
+  (StateT: Type)
+  [BytesFunctor]
+  [Comparse.ParseableSerializeable StateT]
+  [ExecTraceTypes]
+  [ExecTraceTypes.Has Network.ExecEntryT]
+  [ExecTraceTypes.Has (State.ExecEntryT StateT)]
+  [ExecTraceTypes.Has (Compromise.ExecEntryT StateT)]
+  (i: Nat)
+  : Traceful Nat
+:= do
+  PersistentGlobalState.compromise (LocalState StateT) i
+
+public
+def LocalStateCompromised
+  {StateT: Type}
+  [ExecTraceTypes] [ExecTraceTypes.Has (Compromise.ExecEntryT StateT)]
+  (participant: Participant) (state: StateT)
+  (tr: ExecTrace)
+  : Prop
+:=
+  PersistentGlobalState.GlobalStateCompromised ({ participant, state }: LocalState StateT) tr
+
+public
+theorem LocalStateCompromised_le
+  {StateT: Type}
+  [ExecTraceTypes] [ExecTraceTypes.Has (Compromise.ExecEntryT StateT)]
+  (participant: Participant) (state: StateT)
+  (tr1 tr2: ExecTrace)
+  : tr1 ≤ tr2 →
+    LocalStateCompromised participant state tr1 →
+    LocalStateCompromised participant state tr2
+:= by
+  simp [LocalStateCompromised]
+  grind
+
+grind_pattern LocalStateCompromised_le => tr1 ≤ tr2, LocalStateCompromised participant state tr1
+grind_pattern [grind_later] LocalStateCompromised_le => tr1 ≤ tr2, LocalStateCompromised participant state tr1
+
+end Execution
+
+section Proof
+
+namespace Compromise
+
+@[expose]
+public
+def ProofEntryT.internal (StateT: Type): Fin 1 → Type
+  | 0 => PersistentGlobalState.Compromise.ProofEntryT (LocalState StateT)
+
+@[expose, implicit_reducible]
+public
+def ProofEntryT (StateT: Type): Type :=
+  TraceTypes.combine (ProofEntryT.internal StateT)
+
+public
+instance (StateT: Type): ∀ id, ErasableProofEntry (ExecEntryT.internal StateT id) (ProofEntryT.internal StateT id)
+  | 0 => by dsimp only [ExecEntryT.internal, ProofEntryT.internal]; infer_instance
+
+public
+instance (StateT: Type): ErasableProofEntry (ExecEntryT StateT) (ProofEntryT StateT) :=
+  (inferInstance: ErasableProofEntry (ExecTraceTypes.combine (ExecEntryT.internal StateT)) (TraceTypes.combine (ProofEntryT.internal StateT)))
+
+public
+instance (StateT: Type): TraceTypes.HasStep (PersistentGlobalState.Compromise.ProofEntryT (LocalState StateT)) (ProofEntryT StateT) :=
+  inferInstanceAs (TraceTypes.HasStep (ProofEntryT.internal StateT 0) (TraceTypes.combine (ProofEntryT.internal StateT)))
+
+public
+instance [TraceTypes] (StateT: Type): ∀ id, SubTraceInvariant (ProofEntryT.internal StateT id)
+  | 0 => by dsimp only [ProofEntryT.internal]; infer_instance
+
+public
+instance [TraceTypes] (StateT: Type): SubTraceInvariant (ProofEntryT StateT) :=
+  (inferInstance: SubTraceInvariant (TraceTypes.combine (ProofEntryT.internal StateT)))
+
+public
+instance [TraceTypes] (StateT: Type): TraceInvariant.HasStep (PersistentGlobalState.Compromise.ProofEntryT (LocalState StateT)) (ProofEntryT StateT) :=
+  inferInstanceAs (TraceInvariant.HasStep (ProofEntryT.internal StateT 0) (TraceTypes.combine (ProofEntryT.internal StateT)))
+
+public
+instance
+  [TraceInvariant] [BytesFunctor] [BytesInvariants]
+  (StateT: Type)
+  [TraceTypes.Has (ProofEntryT StateT)]
+  [TraceInvariant.Has (ProofEntryT StateT)]
+  : ∀ id, SubBaseAttackerKnowledgeTheorem (ProofEntryT.internal StateT id) (baseAttackerKnowledge.internal StateT id)
+  -- TODO: investigate why infer_instance doesn't work
+  | 0 => by dsimp only [ProofEntryT.internal, baseAttackerKnowledge.internal]; apply PersistentGlobalState.Compromise.baseAttackerKnowledgeTheorem
+
+public
+instance baseAttackerKnowledgeTheorem
+  [TraceInvariant] [BytesFunctor] [BytesInvariants]
+  (StateT: Type)
+  [TraceTypes.Has (ProofEntryT StateT)]
+  [TraceInvariant.Has (ProofEntryT StateT)]
+  : SubBaseAttackerKnowledgeTheorem (ProofEntryT StateT) (baseAttackerKnowledge StateT)
+:= by
+  dsimp only [ProofEntryT, baseAttackerKnowledge]
+  apply instSubBaseAttackerKnowledgeTheoremCombine
+
+end Compromise
+
+public
+def label
+  {StateT: Type}
+  [ExecTraceTypes] [ExecTraceTypes.Has (Compromise.ExecEntryT StateT)]
+  (participant: Participant) (state: StateT)
+:=
+  PersistentGlobalState.label ({ participant, state }: LocalState StateT)
+
+public
+theorem label_isCorrupt
+  {StateT: Type}
+  [ExecTraceTypes] [ExecTraceTypes.Has (Compromise.ExecEntryT StateT)]
+  (participant: Participant) (state: StateT)
+  (tr: ExecTrace)
+  : (label participant state).isCorrupt tr = LocalStateCompromised participant state tr
+:= by
+  grind [label, LocalStateCompromised]
+
+grind_pattern label_isCorrupt => (label participant state).isCorrupt tr
+
+public
+class CompromisableLocalStateInv
+  (StateT: Type)
+  [TraceTypes]
+  [BytesFunctor] [BytesInvariants]
+  [Comparse.ParseableSerializeable StateT]
+  [ExecTraceTypes.Has (Compromise.ExecEntryT StateT)]
+extends
+  LocalStateInv StateT
+where
+  invariant_implies_KnowableBy:
+    ∀ (participant: Participant) (state: StateT) tr,
+      LocalStateInv.invariant participant state tr →
+      Comparse.isWellFormed (Bytes.KnowableBy (label participant state)) state tr
+
+axiom LocalState.isWellFormedLemma
+  [BytesFunctor]
+  {StateT: Type} [Comparse.ParseableSerializeable StateT]
+  (pre: Bytes → τ → Prop) [Comparse.BytesCompatible pre]
+  (x: LocalState StateT) (tr: τ):
+  Comparse.isWellFormed pre x tr = Comparse.isWellFormed pre x.state tr
+
+grind_pattern LocalState.isWellFormedLemma => Comparse.isWellFormed pre x tr
+
+instance
+  [TraceTypes] [BytesFunctor] [BytesInvariants]
+  (StateT: Type)
+  [Comparse.ParseableSerializeable StateT]
+  [ExecTraceTypes.Has (Compromise.ExecEntryT StateT)]
+  [CompromisableLocalStateInv StateT]
+  : PersistentGlobalState.CompromisableGlobalStateInv (LocalState StateT)
+where
+  invariant_implies_KnowableBy := by
+    intro { participant, state } tr
+    have := CompromisableLocalStateInv.invariant_implies_KnowableBy participant state tr
+    simp [label] at this
+    simp [PersistentGlobalState.GlobalStateInv.invariant]
+    grind
+
+@[instance]
+public
+theorem compromise.spec
+  {StateT: Type}
+  [BytesFunctor]
+  [Comparse.ParseableSerializeable StateT]
+  [TraceInvariant]
+  [TraceTypes.Has Network.ProofEntryT]
+  [TraceTypes.Has (State.ProofEntryT StateT)]
+  [TraceTypes.Has (Compromise.ProofEntryT StateT)]
+  [BytesInvariants] [BytesInvariantsProofs]
+  [Comparse.ParseableSerializeable StateT]
+  [CompromisableLocalStateInv StateT]
+  [TraceInvariant.Has Network.ProofEntryT]
+  [TraceInvariant.Has (State.ProofEntryT StateT)]
+  [TraceInvariant.Has (Compromise.ProofEntryT StateT)]
+  (i: Nat)
+  : HoareTriple
+    (compromise StateT i)
+    (fun _ => True)
+    (fun _ _ => True)
+:= by
+  apply HoareTriple.mk
+  unfold compromise
+  step
+  trivial
+
+end Proof
+
+end Compromise
+
+section CompromisableState
+
+namespace CompromisableState
+
+@[expose]
+public
+def ExecEntryT.internal (StateT: Type): Fin 2 → Type
+  | 0 => State.ExecEntryT StateT
+  | 1 => Compromise.ExecEntryT StateT
+
+@[expose, implicit_reducible]
+public
+def ExecEntryT (StateT: Type): Type :=
+  ExecTraceTypes.combine (ExecEntryT.internal StateT)
+
+public
+instance (StateT: Type): ExecTraceTypes.HasStep (State.ExecEntryT StateT) (ExecEntryT StateT) :=
+  inferInstanceAs (ExecTraceTypes.HasStep (ExecEntryT.internal StateT 0) (ExecTraceTypes.combine (ExecEntryT.internal StateT)))
+
+public
+instance (StateT: Type): ExecTraceTypes.HasStep (Compromise.ExecEntryT StateT) (ExecEntryT StateT) :=
+  inferInstanceAs (ExecTraceTypes.HasStep (ExecEntryT.internal StateT 1) (ExecTraceTypes.combine (ExecEntryT.internal StateT)))
+
+public
+def baseAttackerKnowledge.internal [BytesFunctor] [ExecTraceTypes] (StateT: Type): (id: Fin 2) → SubBaseAttackerKnowledge (ExecEntryT.internal StateT id)
+  | 0 => State.baseAttackerKnowledge StateT
+  | 1 => Compromise.baseAttackerKnowledge StateT
+
+public
+def baseAttackerKnowledge [BytesFunctor] [ExecTraceTypes] (StateT: Type): SubBaseAttackerKnowledge (ExecEntryT StateT) :=
+  SubBaseAttackerKnowledge.combine (baseAttackerKnowledge.internal StateT)
+
+@[expose]
+public
+def ProofEntryT.internal (StateT: Type): Fin 2 → Type
+  | 0 => State.ProofEntryT StateT
+  | 1 => Compromise.ProofEntryT StateT
+
+@[expose, implicit_reducible]
+public
+def ProofEntryT (StateT: Type): Type :=
+  TraceTypes.combine (ProofEntryT.internal StateT)
+
+public
+instance (StateT: Type): ∀ id, ErasableProofEntry (ExecEntryT.internal StateT id) (ProofEntryT.internal StateT id)
+  | 0 | 1 => by dsimp only [ExecEntryT.internal, ProofEntryT.internal]; infer_instance
+
+public
+instance (StateT: Type): ErasableProofEntry (ExecEntryT StateT) (ProofEntryT StateT) :=
+  (inferInstance: ErasableProofEntry (ExecTraceTypes.combine (ExecEntryT.internal StateT)) (TraceTypes.combine (ProofEntryT.internal StateT)))
+
+public
+instance (StateT: Type): TraceTypes.HasStep (State.ProofEntryT StateT) (ProofEntryT StateT) :=
+  inferInstanceAs (TraceTypes.HasStep (ProofEntryT.internal StateT 0) (TraceTypes.combine (ProofEntryT.internal StateT)))
+
+public
+instance (StateT: Type): TraceTypes.HasStep (Compromise.ProofEntryT StateT) (ProofEntryT StateT) :=
+  inferInstanceAs (TraceTypes.HasStep (ProofEntryT.internal StateT 1) (TraceTypes.combine (ProofEntryT.internal StateT)))
+
+public
+instance
+  [TraceTypes] [BytesFunctor] [BytesInvariants]
+  (StateT: Type) [Comparse.ParseableSerializeable StateT] [ExecTraceTypes.Has (ExecEntryT StateT)]
+  [CompromisableLocalStateInv StateT]
+  : ∀ id, SubTraceInvariant (ProofEntryT.internal StateT id)
+  | 0 | 1 => by dsimp only [ProofEntryT.internal]; infer_instance
+
+public
+instance
+  [TraceTypes] [BytesFunctor] [BytesInvariants]
+  (StateT: Type) [Comparse.ParseableSerializeable StateT] [ExecTraceTypes.Has (ExecEntryT StateT)]
+  [CompromisableLocalStateInv StateT]
+  : SubTraceInvariant (ProofEntryT StateT)
+:=
+  (inferInstance: SubTraceInvariant (TraceTypes.combine (ProofEntryT.internal StateT)))
+
+public
+instance
+  [TraceTypes] [BytesFunctor] [BytesInvariants]
+  (StateT: Type) [Comparse.ParseableSerializeable StateT] [ExecTraceTypes.Has (ExecEntryT StateT)]
+  [CompromisableLocalStateInv StateT]
+  : TraceInvariant.HasStep (State.ProofEntryT StateT) (ProofEntryT StateT)
+:=
+  inferInstanceAs (TraceInvariant.HasStep (ProofEntryT.internal StateT 0) (TraceTypes.combine (ProofEntryT.internal StateT)))
+
+public
+instance
+  [TraceTypes] [BytesFunctor] [BytesInvariants]
+  (StateT: Type) [Comparse.ParseableSerializeable StateT] [ExecTraceTypes.Has (ExecEntryT StateT)]
+  [CompromisableLocalStateInv StateT]
+  : TraceInvariant.HasStep (Compromise.ProofEntryT StateT) (ProofEntryT StateT)
+:=
+  inferInstanceAs (TraceInvariant.HasStep (ProofEntryT.internal StateT 1) (TraceTypes.combine (ProofEntryT.internal StateT)))
+
+public
+instance
+  [TraceInvariant] [BytesFunctor] [BytesInvariants]
+  (StateT: Type) [Comparse.ParseableSerializeable StateT]
+  [TraceTypes.Has (ProofEntryT StateT)]
+  [CompromisableLocalStateInv StateT]
+  [TraceInvariant.Has (ProofEntryT StateT)]
+  : ∀ id, SubBaseAttackerKnowledgeTheorem (ProofEntryT.internal StateT id) (baseAttackerKnowledge.internal StateT id)
+  -- TODO: investigate why infer_instance doesn't work
+  | 0 => by dsimp only [ProofEntryT.internal, baseAttackerKnowledge.internal]; apply State.baseAttackerKnowledgeTheorem
+  | 1 => by dsimp only [ProofEntryT.internal, baseAttackerKnowledge.internal]; apply Compromise.baseAttackerKnowledgeTheorem
+
+public
+instance baseAttackerKnowledgeTheorem
+  [TraceInvariant] [BytesFunctor] [BytesInvariants]
+  (StateT: Type) [Comparse.ParseableSerializeable StateT]
+  [TraceTypes.Has (ProofEntryT StateT)]
+  [CompromisableLocalStateInv StateT]
+  [TraceInvariant.Has (ProofEntryT StateT)]
+  : SubBaseAttackerKnowledgeTheorem (ProofEntryT StateT) (baseAttackerKnowledge StateT)
+:= by
+  dsimp only [ProofEntryT, baseAttackerKnowledge]
+  apply instSubBaseAttackerKnowledgeTheoremCombine -- infer_instance?
+
+end CompromisableState
+
+end CompromisableState
+
+end DY.PersistentLocalState
