DY/Actions/ProtocolEvent.lean
@@ -1,0 +1,163 @@
+module
+
+public import DY.Trace
+public import DY.Bytes
+import DY.Step.Init
+
+namespace DY.ProtocolEvent
+
+public
+structure ExecEntryT (EventT: Type) where
+  ev: EventT
+
+public
+def baseAttackerKnowledge [BytesFunctor] [ExecTraceTypes] (EventT: Type): SubBaseAttackerKnowledge (ExecEntryT EventT) where
+  attackerKnows _ _ _ := False
+
+public
+abbrev ProofEntryT (EventT: Type) := ExecEntryT EventT
+
+public
+instance (EventT: Type): ErasableProofEntry (ExecEntryT EventT) (ProofEntryT EventT) := ErasableProofEntry.default (ExecEntryT EventT)
+
+public
+class EventInv [TraceTypes] (EventT: Type) where
+  invariant: ProofTrace → EventT → Prop
+
+public
+instance
+  [TraceTypes] (EventT: Type) [EventInv EventT]
+  : SubTraceInvariant (ProofEntryT EventT)
+where
+  invariant tr entry :=
+    EventInv.invariant tr entry.ev
+
+public
+instance baseAttackerKnowledgeTheorem
+  [TraceInvariant] [BytesFunctor] [BytesInvariants]
+  (EventT: Type)
+  [TraceTypes.Has (ProofEntryT EventT)]
+  [EventInv EventT]
+  [TraceInvariant.Has (ProofEntryT EventT)]
+  : SubBaseAttackerKnowledgeTheorem (ProofEntryT EventT) (baseAttackerKnowledge EventT)
+where
+  pf trBefore entry b := by
+    simp [baseAttackerKnowledge]
+
+public
+def _root_.DY.Trace.EventLoggedAt
+  {EventT: Type}
+  [ExecTraceTypes]
+  [ExecTraceTypes.Has (ExecEntryT EventT)]
+  (ev: EventT) (time: Nat)
+  (tr: ExecTrace)
+  : Prop
+:=
+  tr.at_is time (ExecEntryT.mk ev)
+
+public
+theorem _root_.DY.Trace.EventLoggedAt_le
+  {EventT: Type}
+  [ExecTraceTypes]
+  [ExecTraceTypes.Has (ExecEntryT EventT)]
+  (ev: EventT) (time: Nat)
+  (tr1 tr2: ExecTrace)
+  : tr1 ≤ tr2 →
+    tr1.EventLoggedAt ev time →
+    tr2.EventLoggedAt ev time
+:= by
+  grind [Trace.EventLoggedAt]
+
+grind_pattern Trace.EventLoggedAt_le => tr1 ≤ tr2, tr1.EventLoggedAt ev time
+grind_pattern [grind_later] Trace.EventLoggedAt_le => tr1 ≤ tr2, tr1.EventLoggedAt ev time
+
+public
+abbrev _root_.DY.Trace.EventLogged
+  {EventT: Type}
+  [ExecTraceTypes]
+  [ExecTraceTypes.Has (ExecEntryT EventT)]
+  (ev: EventT)
+  (tr: ExecTrace)
+  : Prop
+:=
+  ∃ i, tr.EventLoggedAt ev i
+
+public
+theorem _root_.DY.Trace.EventLoggedAt_imp_EventInv
+  {EventT: Type}
+  [TraceInvariant]
+  [EventInv EventT]
+  [TraceTypes.Has (ProofEntryT EventT)] [TraceInvariant.Has (ProofEntryT EventT)]
+  (ev: EventT)
+  (i: Nat)
+  (tr: ProofTrace)
+  : tr.Invariant →
+    tr.erase.EventLoggedAt ev i →
+    EventInv.invariant (tr.prefix i) ev
+:= by
+  intro h_inv h_ev
+  have := Trace.invariant_at tr i (by grind [Trace.EventLoggedAt, Trace.at_is]) h_inv
+  suffices SubTraceInvariant.invariant (tr.prefix i) (ExecEntryT.mk ev) by
+    simp_all [SubTraceInvariant.invariant]
+  rewrite [← TraceInvariant.Has.inv_commutes]
+  simp [Trace.EventLoggedAt, Trace.at_is, IntoTraceEntry.make, Trace.erase_at, ProofTrace.Entry.erase_eq_imp_exists, ErasableProofEntry.erase] at h_ev
+  grind
+
+public
+def logEvent
+  {EventT: Type}
+  [ExecTraceTypes]
+  [ExecTraceTypes.Has (ExecEntryT EventT)]
+  (ev: EventT): Traceful Unit
+:= do
+  let entry: ExecEntryT EventT := { ev }
+  let _i ← appendEntry entry
+  return ()
+
+@[instance]
+public
+theorem logEvent.spec
+  {EventT: Type}
+  [TraceInvariant]
+  [EventInv EventT]
+  [TraceTypes.Has (ProofEntryT EventT)] [TraceInvariant.Has (ProofEntryT EventT)]
+  (ev: EventT)
+  : HoareTriple
+    (logEvent ev)
+    (fun tr => EventInv.invariant tr ev)
+    (fun _ tr => tr.erase.EventLogged ev)
+:= by
+  apply HoareTriple.mk
+  unfold logEvent
+  dsimp only
+  unfold hoareTriple
+  intro tr h_pre h_inv
+  mark_non_monotone h_pre
+  step with ⟨ fun _ => ExecEntryT.mk ev ⟩ by simp_all [ErasableProofEntry.erase, SubTraceInvariant.invariant]
+  step
+  simp only [Trace.EventLoggedAt]
+  exists _i
+  have := Trace.at_is_erase tr _i (ExecEntryT.mk ev)
+  simp_all [ErasableProofEntry.erase]
+
+public
+def label
+  {EventT: Type}
+  [ExecTraceTypes] [ExecTraceTypes.Has (ExecEntryT EventT)]
+  (ev: EventT)
+  : Label
+where
+  isCorrupt tr := tr.EventLogged ev
+
+public
+theorem label_isCorrupt
+  {EventT: Type}
+  [ExecTraceTypes] [ExecTraceTypes.Has (ExecEntryT EventT)]
+  (ev: EventT) (tr: ExecTrace)
+  : (label ev).isCorrupt tr = tr.EventLogged ev
+:= by
+  rfl
+
+grind_pattern label_isCorrupt => (label ev).isCorrupt tr
+
+end DY.ProtocolEvent
