DY/Comparse.lean
@@ -1,0 +1,143 @@
+module
+
+public import DY.Bytes
+
+namespace DY.Comparse
+
+variable [BytesFunctor]
+
+public
+class ParseableSerializeable (a: Type) where
+  parse: Bytes -> Err a
+  serialize: a -> Bytes
+
+  parse_serialize_inv:
+    ∀ x: a,
+      parse (serialize x) = some x
+
+  serialize_parse_inv:
+    ∀ buf: Bytes, ∀ x: a,
+      parse buf = some x →
+      buf = serialize x
+
+export ParseableSerializeable (parse)
+export ParseableSerializeable (serialize)
+export ParseableSerializeable (parse_serialize_inv)
+export ParseableSerializeable (serialize_parse_inv)
+
+@[simp]
+public
+theorem parse_serialize_inv_grind [ParseableSerializeable a] (x: a):
+  ParseableSerializeable.parse (serialize x) = some x
+  := by
+  exact (parse_serialize_inv x)
+
+grind_pattern parse_serialize_inv_grind => serialize x
+
+public
+def formatRel [ParseableSerializeable a] (buf: Bytes) (x: a) :=
+  buf = serialize x
+
+public
+instance [TraceInvariant] [ParseableSerializeable a]:
+  HoareTriple
+    (parse buf: Err a)
+    (fun _ => True)
+    (fun res _ => formatRel buf res)
+where
+  pf := by
+    simp only [hoareTriple, wp, formatRel, OptionT.run]
+    grind [serialize_parse_inv]
+
+public
+theorem serialize_formatRel [ParseableSerializeable a] (x: a):
+  (formatRel (serialize x) x)
+  := by
+    simp [formatRel]
+
+grind_pattern serialize_formatRel => serialize x
+
+@[grind! .]
+public
+theorem parse_formatRel [ParseableSerializeable a] (b: Bytes):
+  match (parse b: Err a) with
+  | none => True
+  | some x => formatRel b x
+  := by
+    grind [formatRel, serialize_parse_inv]
+
+@[expose]
+public
+def isWellFormed [ParseableSerializeable a] (pre: Bytes → τ → Prop) (x: a) (tr: τ): Prop :=
+  pre (serialize x) tr
+
+public
+theorem isWellFormedFormatRel [ParseableSerializeable a] (pre: Bytes → τ → Prop) (buf: Bytes) (x: a) (tr: τ):
+  formatRel buf x →
+  (pre buf tr = isWellFormed pre x tr)
+  := by
+    grind [isWellFormed, formatRel]
+
+public
+theorem isWellFormedFormatRelBytesWellFormed [TraceTypes] [BytesWellFormed] [ParseableSerializeable a]:
+  ∀ (buf: Bytes) (x: a) (tr: ProofTrace),
+  formatRel buf x →
+  (buf.WellFormed tr = isWellFormed Bytes.WellFormed x tr)
+  := isWellFormedFormatRel Bytes.WellFormed
+
+grind_pattern isWellFormedFormatRelBytesWellFormed => formatRel buf x, buf.WellFormed tr
+
+public
+theorem isWellFormedFormatRelBytesInvariant [TraceTypes] [BytesInvariant] [ParseableSerializeable a]:
+  ∀ (buf: Bytes) (x: a) (tr: ProofTrace),
+  formatRel buf x →
+  (buf.Invariant tr = isWellFormed Bytes.Invariant x tr)
+  := isWellFormedFormatRel Bytes.Invariant
+
+grind_pattern isWellFormedFormatRelBytesInvariant => formatRel buf x, buf.Invariant tr
+
+public
+theorem isWellFormedFormatRelIsPublishable [TraceTypes] [BytesInvariants] [ParseableSerializeable a]:
+  ∀ (buf: Bytes) (x: a) (tr: ProofTrace),
+  formatRel buf x →
+  (buf.Publishable tr = isWellFormed Bytes.Publishable x tr)
+  := isWellFormedFormatRel Bytes.Publishable
+
+grind_pattern isWellFormedFormatRelIsPublishable => formatRel buf x, Bytes.Publishable buf tr
+
+public
+theorem isWellFormedParse [ParseableSerializeable a] (pre: Bytes → τ → Prop) (buf: Bytes) (x: a) (tr: τ):
+  parse buf = some x →
+  pre buf tr →
+  isWellFormed pre x tr
+  := by
+    grind [isWellFormed, serialize_parse_inv]
+
+public
+class BytesCompatible (pre: Bytes → τ → Prop) where
+  dummy: Unit
+
+public
+instance [TraceTypes] [BytesWellFormed]: BytesCompatible Bytes.WellFormed where
+  dummy := ()
+
+public
+instance [TraceTypes] [BytesInvariant]: BytesCompatible Bytes.Invariant where
+  dummy := ()
+
+public
+instance [TraceTypes] [BytesInvariants]: BytesCompatible Bytes.Publishable where
+  dummy := ()
+
+public
+instance [TraceTypes] [BytesInvariants] (l: Label): BytesCompatible (Bytes.KnowableBy l) where
+  dummy := ()
+
+public
+instance [ExecTraceTypes] [BaseAttackerKnowledge] [AttackerKnowledge]: BytesCompatible Bytes.AttackerKnows where
+  dummy := ()
+
+public
+axiom comparseMetaProgramExists {a: Type}: ParseableSerializeable a
+
+end DY.Comparse
