DY/Trace.lean
@@ -1,5 +1,8 @@
 module
 
 public import DY.Trace.Basic
+public import DY.Trace.BaseAttackerKnowledge
+public import DY.Trace.Invariant
+public import DY.Trace.BaseAttackerKnowledgeTheorem
 public import DY.Trace.Manipulation
 public meta import DY.Trace.Grind
