DY/Trace/BaseAttackerKnowledge.lean
@@ -1,0 +1,125 @@
+module
+
+public import DY.Bytes.Basic
+public import DY.Trace.Basic
+import all DY.Trace.Basic
+
+namespace DY
+
+public
+structure SubBaseAttackerKnowledge [BytesFunctor] [ExecTraceTypes] (ExecEntryT: Type) where
+  attackerKnows: ExecTrace → ExecEntryT → Bytes → Prop
+
+public
+class BaseAttackerKnowledge [BytesFunctor] [ExecTraceTypes] where
+  attackerKnows: SubBaseAttackerKnowledge ExecTrace.Entry
+
+public
+class BaseAttackerKnowledge.Has
+  [BytesFunctor] [ExecTraceTypes]
+  [BaseAttackerKnowledge]
+  {ExecEntryT: Type}
+  [ExecTraceTypes.Has ExecEntryT]
+  (sub: SubBaseAttackerKnowledge ExecEntryT)
+where
+  pf: ∀ tr entry b,
+    sub.attackerKnows tr entry b →
+    BaseAttackerKnowledge.attackerKnows.attackerKnows tr (ExecTraceTypes.Has.inj entry) b
+
+public
+class BaseAttackerKnowledge.HasStep
+  [BytesFunctor] [ExecTraceTypes]
+  [BaseAttackerKnowledge]
+  {ExecEntryT1: Type} {ExecEntryT2: semiOutParam Type}
+  [ExecTraceTypes.HasStep ExecEntryT1 ExecEntryT2]
+  (sub1: SubBaseAttackerKnowledge ExecEntryT1)
+  (sub2: semiOutParam (SubBaseAttackerKnowledge ExecEntryT2))
+where
+  pf: ∀ tr entry b,
+    sub1.attackerKnows tr entry b →
+    sub2.attackerKnows tr (ExecTraceTypes.HasStep.inj entry) b
+
+public
+instance instBaseAttackerKnowledgeHasItself
+  [BytesFunctor] [ExecTraceTypes]
+  [BaseAttackerKnowledge]
+  : BaseAttackerKnowledge.Has (BaseAttackerKnowledge.attackerKnows)
+where
+  pf := by simp [ExecTraceTypes.Has.inj]
+
+public
+instance instBaseAttackerKnowledgeHasStep
+  [BytesFunctor] [ExecTraceTypes]
+  [BaseAttackerKnowledge]
+  {ExecEntryT1 ExecEntryT2: Type}
+  [ExecTraceTypes.HasStep ExecEntryT1 ExecEntryT2]
+  [ExecTraceTypes.Has ExecEntryT2]
+  (sub1: SubBaseAttackerKnowledge ExecEntryT1)
+  (sub2: SubBaseAttackerKnowledge ExecEntryT2)
+  [BaseAttackerKnowledge.HasStep sub1 sub2]
+  [BaseAttackerKnowledge.Has sub2]
+  : BaseAttackerKnowledge.Has sub1
+where
+  pf := by
+    have := BaseAttackerKnowledge.HasStep.pf (sub1 := sub1) (sub2 := sub2)
+    have := BaseAttackerKnowledge.Has.pf (sub := sub2)
+    simp [ExecTraceTypes.Has.inj]
+    grind
+
+public
+def SubBaseAttackerKnowledge.combine
+  [BytesFunctor] [ExecTraceTypes]
+  {n: Nat}
+  {Types: Fin n → Type}
+  (subs: (id: Fin n) → SubBaseAttackerKnowledge (Types id))
+  : SubBaseAttackerKnowledge (ExecTraceTypes.combine Types)
+where
+  attackerKnows := fun tr {id, entry} b =>
+    (subs id).attackerKnows tr entry b
+
+public
+instance instBaseAttackerKnowledgeCombineHasStep
+  [BytesFunctor] [ExecTraceTypes]
+  [BaseAttackerKnowledge]
+  {n: Nat}
+  {Types: Fin n → Type}
+  (subs: (id: Fin n) → SubBaseAttackerKnowledge (Types id))
+  (id: Fin n)
+  : BaseAttackerKnowledge.HasStep (subs id) (SubBaseAttackerKnowledge.combine subs)
+where
+  pf := by
+    simp [ExecTraceTypes.HasStep.inj, SubBaseAttackerKnowledge.combine]
+
+public
+def Trace.BaseAttackerKnows
+  [BytesFunctor] [ExecTraceTypes] [BaseAttackerKnowledge]
+  (tr: ExecTrace) (b: Bytes)
+  : Prop
+:=
+  match tr with
+  | .nil => False
+  | .snoc trBefore entry =>
+    BaseAttackerKnowledge.attackerKnows.attackerKnows trBefore entry b ∨
+    Trace.BaseAttackerKnows trBefore b
+
+public
+def Trace.prove_BaseAttackerKnows
+  [BytesFunctor] [ExecTraceTypes] [BaseAttackerKnowledge]
+  {ExecEntryT: Type}
+  [ExecTraceTypes.Has ExecEntryT]
+  (sub: SubBaseAttackerKnowledge ExecEntryT)
+  [BaseAttackerKnowledge.Has sub]
+  (tr: ExecTrace) (entry: ExecEntryT) (b: Bytes)
+  (time: Nat)
+  : tr.at_is time entry →
+    sub.attackerKnows (tr.prefix time) entry b →
+    Trace.BaseAttackerKnows tr b
+:= by
+  induction tr
+  · grind [Trace.at_is, Trace.length]
+  rename_i tr entry' ih
+  have := BaseAttackerKnowledge.Has.pf (sub := sub) tr entry b
+  simp_all [Trace.prefix, Trace.length, Trace.at_is, Trace.at, IntoTraceEntry.make, Trace.BaseAttackerKnows]
+  grind
+
+end DY
