DY/Trace/BaseAttackerKnowledgeTheorem.lean
@@ -1,0 +1,74 @@
+module
+
+public import DY.Bytes.Basic
+public import DY.Bytes.Invariants
+public import DY.Trace.Basic
+public import DY.Trace.Invariant
+public import DY.Trace.BaseAttackerKnowledge
+import all DY.Trace.Invariant
+import all DY.Trace.BaseAttackerKnowledge
+
+namespace DY
+
+public
+class SubBaseAttackerKnowledgeTheorem
+  [TraceInvariant]
+  [BytesFunctor] [BytesInvariants]
+  {ExecEntryT: Type}
+  (ProofEntryT: Type)
+  [ErasableProofEntry ExecEntryT ProofEntryT]
+  [SubTraceInvariant ProofEntryT]
+  [TraceTypes.Has ProofEntryT] [TraceInvariant.Has ProofEntryT]
+  (att: SubBaseAttackerKnowledge ExecEntryT)
+where
+  pf: ∀ trBefore (entry: ProofEntryT) (b: Bytes),
+    SubTraceInvariant.invariant trBefore entry →
+    att.attackerKnows trBefore.erase (ErasableProofEntry.erase entry) b →
+    b.Publishable trBefore -- could also be `b.Publishable (trBefore.append entry)` if needed
+
+public
+class BaseAttackerKnowledgeTheorem
+  [TraceInvariant]
+  [BytesFunctor] [BytesInvariants]
+  [BaseAttackerKnowledge]
+where
+  pf: SubBaseAttackerKnowledgeTheorem ProofTrace.Entry BaseAttackerKnowledge.attackerKnows
+
+public
+instance instSubBaseAttackerKnowledgeTheoremCombine
+  [TraceInvariant]
+  [BytesFunctor] [BytesInvariants]
+  {n: Nat}
+  {ExecTypes: Fin n → Type} {ProofTypes: Fin n → Type}
+  [∀ id, ErasableProofEntry (ExecTypes id) (ProofTypes id)]
+  [∀ id, SubTraceInvariant (ProofTypes id)]
+  [TraceTypes.Has (TraceTypes.combine ProofTypes)] [TraceInvariant.Has (TraceTypes.combine ProofTypes)]
+  (atts: (id: Fin n) → SubBaseAttackerKnowledge (ExecTypes id))
+  [attThms: (id: Fin n) → SubBaseAttackerKnowledgeTheorem (ProofTypes id) (atts id)]
+  : SubBaseAttackerKnowledgeTheorem (TraceTypes.combine ProofTypes) (SubBaseAttackerKnowledge.combine atts)
+where
+  pf := fun trBefore { id, entry } b =>
+    (attThms id).pf trBefore entry b
+
+public
+theorem Trace.BaseAttackerKnows_implies_Publishable
+  [TraceInvariant]
+  [BytesFunctor] [BytesInvariants] [BytesInvariantsProofs]
+  [BaseAttackerKnowledge] [BaseAttackerKnowledgeTheorem]
+  (tr: ProofTrace) (b: Bytes)
+  : Trace.Invariant tr →
+    Trace.BaseAttackerKnows tr.erase b →
+    b.Publishable tr
+:= by
+  induction tr
+  · simp [Trace.BaseAttackerKnows, Trace.erase]
+  rename_i trBefore entry ih
+  have h_le: trBefore ≤ trBefore.snoc entry := by apply Trace.le.extend; apply Trace.le.equal
+  simp only [Trace.Invariant, Trace.BaseAttackerKnows, Trace.erase]
+  intro h_inv h_att
+  cases h_att
+  · have := BaseAttackerKnowledgeTheorem.pf.pf trBefore entry b (by grind [ProofTrace.Entry.Invariant]) (by grind [ProofTrace.Entry.erase])
+    grind
+  · grind
+
+end DY
