DY/Trace/Invariant.lean
@@ -1,0 +1,416 @@
+module
+
+public import DY.Trace.Basic
+import all DY.Trace.Basic
+public meta import DY.Trace.Grind
+
+namespace DY
+
+public
+class ErasableProofEntry (ExecEntryT: outParam Type) (ProofEntryT: Type) where
+  erase: ProofEntryT → ExecEntryT
+
+public
+abbrev ErasableProofEntry.default (ExecEntryT: Type): ErasableProofEntry ExecEntryT ExecEntryT where
+  erase x := x
+
+public
+class TraceTypes extends ExecTraceTypes where
+  ProofT: Type
+  tc: ErasableProofEntry ExecT ProofT
+
+@[expose]
+public
+def ProofTrace.Entry [TraceTypes] := TraceTypes.ProofT
+
+public
+instance [TraceTypes]: ErasableProofEntry ExecTrace.Entry ProofTrace.Entry where
+  erase entry := TraceTypes.tc.erase entry
+
+public
+abbrev ProofTrace [TraceTypes] := Trace ProofTrace.Entry
+
+@[expose]
+public
+def ProofTrace.Entry.erase
+  [TraceTypes]
+  (entry: ProofTrace.Entry)
+  : ExecTrace.Entry
+:=
+  ErasableProofEntry.erase entry
+
+public
+def Trace.erase
+  [TraceTypes]
+  (tr: ProofTrace)
+  : ExecTrace
+:=
+  match tr with
+  | .nil => .nil
+  | .snoc trBefore entry => .snoc trBefore.erase entry.erase
+
+public
+theorem Trace.erase_le
+  [TraceTypes]
+  (tr1 tr2: ProofTrace)
+  : tr1 ≤ tr2 →
+    tr1.erase ≤ tr2.erase
+:= by
+  intro h_le
+  induction h_le
+  · apply Trace.le.equal
+  · apply Trace.le.extend
+    assumption
+
+grind_pattern Trace.erase_le => tr1 ≤ tr2, tr1.erase
+grind_pattern [grind_later] Trace.erase_le => tr1 ≤ tr2, tr1.erase
+
+public
+theorem Trace.erase_length
+  [TraceTypes]
+  (tr: ProofTrace)
+  : tr.erase.length = tr.length
+:= by
+  induction tr <;>
+  simp_all [Trace.length, Trace.erase]
+
+grind_pattern Trace.erase_length => tr.erase.length
+
+public
+def Trace.erase_at
+  [TraceTypes]
+  (tr: ProofTrace)
+  (i: Nat) (h_i: i < tr.erase.length)
+  : tr.erase.at i h_i = (tr.at i (Trace.erase_length tr ▸ h_i)).erase
+:= by
+  induction tr <;>
+  simp only [Trace.at, Trace.erase]
+  · grind
+  split <;>
+  grind [Trace.erase_length]
+
+-- TODO test coercion
+example [TraceTypes]: Coe ProofTrace ExecTrace where
+  coe tr := tr.erase
+
+public
+class TraceTypes.Has
+  [TraceTypes]
+  {ExecEntryT: outParam Type} (ProofEntryT: Type)
+  [ErasableProofEntry ExecEntryT ProofEntryT]
+  extends ExecTraceTypes.Has ExecEntryT
+where
+  proofInj: ProofEntryT → ProofTrace.Entry
+  proofProj: ProofTrace.Entry → Option ProofEntryT
+  proof_inj_proj_eq: ∀ x y, (proofProj x = some y) = (x = proofInj y)
+  proofProj_none_eq_erase: ∀ x, ((proofProj x: Option ProofEntryT) = none) = ((proj x.erase: Option ExecEntryT) = none)
+  erase_commutes: ∀ entry, (proofInj entry).erase = inj (ErasableProofEntry.erase entry)
+
+public
+class TraceTypes.HasStep
+  {ExecEntryT1 ExecEntryT2: outParam Type}
+  (ProofEntryT1: Type) (ProofEntryT2: semiOutParam Type)
+  [ErasableProofEntry ExecEntryT1 ProofEntryT1]
+  [ErasableProofEntry ExecEntryT2 ProofEntryT2]
+  extends ExecTraceTypes.HasStep ExecEntryT1 ExecEntryT2
+where
+  proofInj: ProofEntryT1 → ProofEntryT2
+  proofProj: ProofEntryT2 → Option ProofEntryT1
+  proof_inj_proj_eq: ∀ x y, (proofProj x = some y) = (x = proofInj y)
+  proofProj_none_eq_erase: ∀ x, ((proofProj x: Option ProofEntryT1) = none) = ((proj (ErasableProofEntry.erase x): Option ExecEntryT1) = none)
+  erase_commutes: ∀ entry, ErasableProofEntry.erase (proofInj entry) = inj (ErasableProofEntry.erase entry)
+
+public
+instance instTraceTypesHasItself
+  [TraceTypes]
+  : TraceTypes.Has ProofTrace.Entry
+where
+  proofInj entry := entry
+  proofProj entry := some entry
+  proof_inj_proj_eq := by grind
+  proofProj_none_eq_erase := by simp [ExecTraceTypes.Has.proj]
+  erase_commutes := by simp [ExecTraceTypes.Has.inj, ProofTrace.Entry.erase]
+
+public
+instance instTraceTypesHasStep
+  [TraceTypes]
+  {ExecEntryT1 ExecEntryT2: Type}
+  (ProofEntryT1 ProofEntryT2: Type)
+  [ErasableProofEntry ExecEntryT1 ProofEntryT1]
+  [ErasableProofEntry ExecEntryT2 ProofEntryT2]
+  [TraceTypes.HasStep ProofEntryT1 ProofEntryT2]
+  [TraceTypes.Has ProofEntryT2]
+  : TraceTypes.Has ProofEntryT1
+where
+  proofInj entry := TraceTypes.Has.proofInj (TraceTypes.HasStep.proofInj (ProofEntryT2 := ProofEntryT2) entry)
+  proofProj entry :=
+    match TraceTypes.Has.proofProj (ProofEntryT := ProofEntryT2) entry with
+    | none => none
+    | some y => TraceTypes.HasStep.proofProj y
+
+  proof_inj_proj_eq x y := by
+    have := TraceTypes.Has.proof_inj_proj_eq (ProofEntryT := ProofEntryT2) x
+    have := TraceTypes.HasStep.proof_inj_proj_eq (ProofEntryT1 := ProofEntryT1) (ProofEntryT2 := ProofEntryT2)
+    grind
+  proofProj_none_eq_erase := by
+    intro x
+    have := ExecTraceTypes.Has.inj_proj_eq (ExecEntryT := ExecEntryT2)
+    have := TraceTypes.Has.proof_inj_proj_eq (ProofEntryT := ProofEntryT2)
+    have := TraceTypes.Has.proofProj_none_eq_erase (ProofEntryT := ProofEntryT2)
+    have := TraceTypes.HasStep.proofProj_none_eq_erase (ProofEntryT1 := ProofEntryT1) (ProofEntryT2 := ProofEntryT2)
+    have := TraceTypes.Has.erase_commutes (ProofEntryT := ProofEntryT2)
+    simp [ExecTraceTypes.Has.proj]
+    grind
+  erase_commutes := by
+    have := TraceTypes.Has.erase_commutes (ProofEntryT := ProofEntryT2)
+    have := TraceTypes.HasStep.erase_commutes (ProofEntryT1 := ProofEntryT1) (ProofEntryT2 := ProofEntryT2)
+    simp [ExecTraceTypes.Has.inj]
+    grind
+
+public
+instance [TraceTypes] {ExecEntryT: Type} (ProofEntryT: Type) [ErasableProofEntry ExecEntryT ProofEntryT] [TraceTypes.Has ProofEntryT]: IntoTraceEntry ProofEntryT ProofTrace.Entry where
+  make entry := TraceTypes.Has.proofInj entry
+
+public
+structure TraceTypes.combine {n: Nat} (ProofTypes: Fin n → Type): Type where
+  id: Fin n
+  entry: ProofTypes id
+
+public
+instance
+  {n: Nat}
+  (ExecTypes: Fin n → Type)
+  (ProofTypes: Fin n → Type)
+  [∀ id, ErasableProofEntry (ExecTypes id) (ProofTypes id)]
+  : ErasableProofEntry (ExecTraceTypes.combine ExecTypes) (TraceTypes.combine ProofTypes)
+where
+  erase := fun { id, entry } => { id, entry := ErasableProofEntry.erase entry }
+
+public
+instance instTraceTypesCombineHasStep
+  {n: Nat}
+  (ExecTypes: Fin n → Type)
+  (ProofTypes: Fin n → Type)
+  [∀ id, ErasableProofEntry (ExecTypes id) (ProofTypes id)]
+  (id: Fin n):
+  TraceTypes.HasStep (ProofTypes id) (TraceTypes.combine ProofTypes)
+where
+  proofInj entry := { id, entry }
+  proofProj entry :=
+    if h: entry.id = id then
+      some (h ▸ entry.entry)
+    else
+      none
+  proof_inj_proj_eq x y := by
+    cases x
+    grind
+  proofProj_none_eq_erase x := by
+    simp [ExecTraceTypes.HasStep.proj, ErasableProofEntry.erase]
+  erase_commutes _ := rfl
+
+public
+theorem ProofTrace.Entry.erase_eq_imp_exists
+  [TraceTypes]
+  {ExecEntryT ProofEntryT: Type}
+  [ErasableProofEntry ExecEntryT ProofEntryT]
+  [TraceTypes.Has ProofEntryT]
+  {entry: ProofTrace.Entry}
+  {result: ExecEntryT}
+  : entry.erase = ExecTraceTypes.Has.inj result ↔ (
+      ∃ result': ProofEntryT,
+      entry = TraceTypes.Has.proofInj result' ∧
+      ErasableProofEntry.erase result' = result
+    )
+:= by
+  cases h: (TraceTypes.Has.proofProj entry: Option ProofEntryT)
+  · have := TraceTypes.Has.proofProj_none_eq_erase (ProofEntryT := ProofEntryT) entry
+    rewrite [← ExecTraceTypes.Has.inj_proj_eq]
+    simp_all only [reduceCtorEq, false_iff, not_exists]
+    intro x
+    have := TraceTypes.Has.proof_inj_proj_eq entry x
+    grind
+  · rename_i result'
+    rewrite [TraceTypes.Has.proof_inj_proj_eq] at h
+    grind [TraceTypes.Has.erase_commutes]
+
+public
+theorem Trace.append_erase
+  [TraceTypes]
+  {ExecEntryT ProofEntryT: Type}
+  [ErasableProofEntry ExecEntryT ProofEntryT]
+  [TraceTypes.Has ProofEntryT]
+  (tr: ProofTrace) (entry: ProofEntryT)
+  : (tr.append entry).erase = tr.erase.append (ErasableProofEntry.erase entry)
+:= by
+  simp [Trace.append, Trace.erase, IntoTraceEntry.make, TraceTypes.Has.erase_commutes]
+
+public
+theorem Trace.at_is_imp_proofProj_at
+  [TraceTypes]
+  {ExecEntryT ProofEntryT: Type}
+  [ErasableProofEntry ExecEntryT ProofEntryT]
+  [TraceTypes.Has ProofEntryT]
+  (tr: ProofTrace) (i: Nat) (entry: ProofEntryT)
+  : tr.at_is i entry →
+    exists h: i < tr.length,
+    TraceTypes.Has.proofProj (tr.at i h) = some entry
+:= by
+  simp only [Trace.at_is, IntoTraceEntry.make]
+  intro ⟨ h1, h2 ⟩
+  exists h1
+  grind [TraceTypes.Has.proof_inj_proj_eq]
+
+public
+theorem Trace.at_is_erase
+  [TraceTypes]
+  {ExecEntryT ProofEntryT: Type}
+  [ErasableProofEntry ExecEntryT ProofEntryT]
+  [TraceTypes.Has ProofEntryT]
+  (tr: ProofTrace) (i: Nat) (entry: ProofEntryT)
+  : tr.at_is i entry →
+    tr.erase.at_is i (ErasableProofEntry.erase entry)
+:= by
+  simp only [Trace.at_is, IntoTraceEntry.make]
+  intro ⟨ h1, h2 ⟩
+  simp_all [Trace.erase_at, TraceTypes.Has.erase_commutes]
+  grind
+
+-- Invariant
+
+public
+class SubTraceInvariant [TraceTypes] {ExecEntryT: outParam Type} (ProofEntryT: Type) [ErasableProofEntry ExecEntryT ProofEntryT] where
+  invariant: ProofTrace → ProofEntryT → Prop
+
+public
+class TraceInvariant extends TraceTypes where
+  tc_inv: SubTraceInvariant ProofTrace.Entry
+
+public
+instance [TraceInvariant]: SubTraceInvariant ProofTrace.Entry where
+  invariant := TraceInvariant.tc_inv.invariant
+
+public
+def ProofTrace.Entry.Invariant
+  [TraceInvariant]
+  (trBefore: ProofTrace)
+  (entry: ProofTrace.Entry)
+  : Prop
+:=
+  SubTraceInvariant.invariant trBefore entry
+
+public
+def Trace.Invariant
+  [TraceInvariant]
+  (tr: ProofTrace)
+  : Prop
+:=
+  match tr with
+  | .nil => True
+  | .snoc trBefore entry =>
+    trBefore.Invariant ∧
+    entry.Invariant trBefore
+
+public
+class TraceInvariant.Has
+  [TraceInvariant]
+  {ExecEntryT: outParam Type}
+  (ProofEntryT: Type)
+  [ErasableProofEntry ExecEntryT ProofEntryT]
+  [TraceTypes.Has ProofEntryT]
+  [SubTraceInvariant ProofEntryT]
+where
+  inv_commutes: ∀ trBefore: ProofTrace, ∀ entry: ProofEntryT, (TraceTypes.Has.proofInj entry).Invariant trBefore = SubTraceInvariant.invariant trBefore entry
+
+public
+class TraceInvariant.HasStep
+  [TraceTypes]
+  {ExecEntryT1 ExecEntryT2: outParam Type}
+  (ProofEntryT1 ProofEntryT2: Type)
+  [ErasableProofEntry ExecEntryT1 ProofEntryT1]
+  [ErasableProofEntry ExecEntryT2 ProofEntryT2]
+  [TraceTypes.HasStep ProofEntryT1 ProofEntryT2]
+  [SubTraceInvariant ProofEntryT1]
+  [SubTraceInvariant ProofEntryT2]
+where
+  inv_commutes: ∀ trBefore: ProofTrace, ∀ entry: ProofEntryT1, SubTraceInvariant.invariant trBefore (TraceTypes.HasStep.proofInj entry: ProofEntryT2) = SubTraceInvariant.invariant trBefore entry
+
+public
+instance instTraceInvariantHasItself
+  [TraceInvariant]
+  : TraceInvariant.Has ProofTrace.Entry
+where
+  inv_commutes := by simp [TraceTypes.Has.proofInj, ProofTrace.Entry.Invariant]
+
+public
+instance instTraceInvariantHasStep
+  [TraceInvariant]
+  {ExecEntryT1 ProofEntryT1: Type}
+  {ExecEntryT2 ProofEntryT2: Type}
+  [ErasableProofEntry ExecEntryT1 ProofEntryT1]
+  [ErasableProofEntry ExecEntryT2 ProofEntryT2]
+  [TraceTypes.HasStep ProofEntryT1 ProofEntryT2]
+  [TraceTypes.Has ProofEntryT2]
+  [SubTraceInvariant ProofEntryT1]
+  [SubTraceInvariant ProofEntryT2]
+  [TraceInvariant.HasStep ProofEntryT1 ProofEntryT2]
+  [TraceInvariant.Has ProofEntryT2]
+  : TraceInvariant.Has ProofEntryT1
+where
+  inv_commutes := by
+    have := TraceInvariant.HasStep.inv_commutes (ProofEntryT1 := ProofEntryT1) (ProofEntryT2 := ProofEntryT2)
+    have := TraceInvariant.Has.inv_commutes (ProofEntryT := ProofEntryT2)
+    simp_all [TraceTypes.Has.proofInj]
+
+public
+instance SubTraceInvariant.combine
+  [TraceTypes]
+  {n: Nat}
+  {ExecTypes: Fin n → Type}
+  {ProofTypes: Fin n → Type}
+  [∀ id, ErasableProofEntry (ExecTypes id) (ProofTypes id)]
+  [∀ id, SubTraceInvariant (ProofTypes id)]
+  : SubTraceInvariant (TraceTypes.combine ProofTypes)
+where
+  invariant := fun trBefore { id := _, entry } =>
+    SubTraceInvariant.invariant trBefore entry
+
+public
+instance instTraceInvariantCombineHasStep
+  [TraceTypes]
+  {n: Nat}
+  {ExecTypes: Fin n → Type}
+  (ProofTypes: Fin n → Type)
+  [∀ id, ErasableProofEntry (ExecTypes id) (ProofTypes id)]
+  [∀ id, SubTraceInvariant (ProofTypes id)]
+  (id: Fin n)
+  : TraceInvariant.HasStep (ProofTypes id) (TraceTypes.combine ProofTypes)
+where
+  inv_commutes trBefore entry := by rfl
+
+public
+theorem Trace.invariant_append
+  [TraceInvariant]
+  {ExecEntryT ProofEntryT: Type}
+  [ErasableProofEntry ExecEntryT ProofEntryT]
+  [TraceTypes.Has ProofEntryT]
+  [SubTraceInvariant ProofEntryT]
+  [TraceInvariant.Has ProofEntryT]
+  (tr: ProofTrace) (entry: ProofEntryT)
+  : (tr.append entry).Invariant = (tr.Invariant ∧ SubTraceInvariant.invariant tr entry)
+:= by
+  have := TraceInvariant.Has.inv_commutes (ProofEntryT := ProofEntryT)
+  simp_all [Trace.Invariant, Trace.append, IntoTraceEntry.make]
+
+public
+theorem Trace.invariant_at
+  [TraceInvariant]
+  (tr: ProofTrace)
+  (i: Nat)
+  (h_i: i < tr.length)
+  : tr.Invariant →
+    (tr.at i h_i).Invariant (tr.prefix i)
+:= by
+  fun_induction Trace.at <;>
+  grind [Trace.Invariant, Trace.prefix, Trace.length]
+
+end DY
